progs/entail_examples.v
@@ -1,0 +1,2651 @@
+Load loadpath.
+Require Import floyd.proofauto.
+Require Import progs.list_dt.
+Require Import progs.queue.
+Local Open Scope logic.
+
+Instance QS: listspec t_struct_elem _next. 
+Proof. eapply mk_listspec; reflexivity. Defined.
+
+Lemma isnil: forall {T: Type} (s: list T), {s=nil}+{s<>nil}.
+Proof. intros. destruct s; [left|right]; auto. intro Hx; inv Hx. Qed.
+
+Definition link := field_mapsto Tsh t_struct_elem _next.
+Definition link_ := field_mapsto_ Tsh t_struct_elem _next.
+
+Definition fifo (contents: list val) (p: val) : mpred:=
+  EX ht: (val*val), let (hd,tl) := ht in
+      field_mapsto Tsh t_struct_fifo _head p hd *
+      field_mapsto Tsh t_struct_fifo _tail p tl *
+      if isnil contents
+      then (!!(hd=nullval) && emp)
+      else (EX prefix: list val, 
+              !!(contents = prefix++tl::nil)
+            &&  (links QS Tsh prefix hd tl * link tl nullval)).
+
+Definition elemrep (rep: elemtype QS) (p: val) : mpred :=
+  field_mapsto Tsh t_struct_elem _a p (Vint (fst rep)) * 
+  (field_mapsto Tsh t_struct_elem _b p (Vint (snd rep)) *
+   (field_mapsto_ Tsh t_struct_elem _next p)).
+
+Lemma goal_1 :
+name _Q ->
+name _h ->
+forall (q : val) (contents : list val) (hd tl : val),
+let Delta :=
+  @abbreviate tycontext
+    (initialized _h
+       (@PTree.Node (type * bool)
+          (@PTree.Node (type * bool) (@PTree.Leaf (type * bool))
+             (@None (type * bool))
+             (@PTree.Node (type * bool) (@PTree.Leaf (type * bool))
+                (@None (type * bool))
+                (@PTree.Node (type * bool)
+                   (@PTree.Node (type * bool) (@PTree.Leaf (type * bool))
+                      (@Some (type * bool) (tptr t_struct_elem, false))
+                      (@PTree.Leaf (type * bool))) (@None (type * bool))
+                   (@PTree.Leaf (type * bool))))) (@None (type * bool))
+          (@PTree.Node (type * bool) (@PTree.Leaf (type * bool))
+             (@None (type * bool))
+             (@PTree.Node (type * bool)
+                (@PTree.Node (type * bool)
+                   (@PTree.Node (type * bool) (@PTree.Leaf (type * bool))
+                      (@Some (type * bool) (tptr t_struct_fifo, true))
+                      (@PTree.Leaf (type * bool))) (@None (type * bool))
+                   (@PTree.Leaf (type * bool))) (@None (type * bool))
+                (@PTree.Leaf (type * bool)))), PTree.empty type, tint,
+       @PTree.Node global_spec
+         (@PTree.Node global_spec
+            (@PTree.Node global_spec
+               (@PTree.Node global_spec (@PTree.Leaf global_spec)
+                  (@Some global_spec
+                     (Global_func
+                        (WITH _ : unit PRE  [(1%positive, tptr tvoid),
+                         (2%positive, tptr tvoid), (3%positive, tuint),
+                         (4%positive, tuint)](fun _ : environ => !!False)
+                         POST  [tvoid](fun _ : environ => !!False))))
+                  (@PTree.Node global_spec (@PTree.Leaf global_spec)
+                     (@Some global_spec
+                        (Global_func
+                           (WITH  p0 : val * list val, p : val PRE 
+                            [(_Q, tptr t_struct_fifo),
+                            (_p, tptr t_struct_elem)]
+                            (let (q0, contents0) := p0 in
+                             PROP  ()
+                             LOCAL  (`(@eq val q0) (eval_id _Q);
+                             `(@eq val p) (eval_id _p))
+                             SEP  (`(fifo contents0 q0); `(link_ p))) POST 
+                            [tvoid]
+                            (let (q0, contents0) := p0 in
+                             `(fifo (contents0 ++ p :: @nil val) q0)))))
+                     (@PTree.Leaf global_spec))) (@None global_spec)
+               (@PTree.Node global_spec
+                  (@PTree.Node global_spec (@PTree.Leaf global_spec)
+                     (@Some global_spec
+                        (Global_func
+                           (WITH _ : unit PRE  []
+                            (fun _ : environ => @emp mpred Nveric Sveric)
+                            POST  [tptr t_struct_fifo]
+                            `(fifo (@nil val)) retval)))
+                     (@PTree.Leaf global_spec)) (@None global_spec)
+                  (@PTree.Node global_spec (@PTree.Leaf global_spec)
+                     (@Some global_spec
+                        (Global_func
+                           (WITH  a : int, b : int PRE  [(_a, tint),
+                            (_b, tint)]
+                            PROP  ()
+                            LOCAL  (`(@eq val (Vint a)) (eval_id _a);
+                            `(@eq val (Vint b)) (eval_id _b))  SEP() POST 
+                            [tptr t_struct_elem]`(elemrep (a, b)) retval)))
+                     (@PTree.Leaf global_spec)))) (@None global_spec)
+            (@PTree.Node global_spec
+               (@PTree.Node global_spec (@PTree.Leaf global_spec)
+                  (@Some global_spec
+                     (Global_func
+                        (WITH n : int PRE  [(1%positive, tint)]
+                         PROP  (4 <= Int.signed n)
+                         LOCAL  (`(@eq val (Vint n)) (eval_id 1%positive))
+                         SEP() POST  [tptr tvoid]`(memory_block Tsh n) retval)))
+                  (@PTree.Leaf global_spec)) (@None global_spec)
+               (@PTree.Leaf global_spec))) (@None global_spec)
+         (@PTree.Node global_spec
+            (@PTree.Node global_spec
+               (@PTree.Node global_spec (@PTree.Leaf global_spec)
+                  (@Some global_spec
+                     (Global_func
+                        (WITH _ : unit PRE  [(1%positive, tptr tschar),
+                         (2%positive, tint)](fun _ : environ => !!False)
+                         POST  [tint](fun _ : environ => !!False))))
+                  (@PTree.Node global_spec (@PTree.Leaf global_spec)
+                     (@Some global_spec
+                        (Global_func
+                           (WITH  q0 : val, contents0 : list val PRE 
+                            [(_Q, tptr t_struct_fifo)]
+                            PROP  ()
+                            LOCAL  (`(@eq val q0) (eval_id _Q))
+                            SEP  (`(fifo contents0 q0)) POST  [tint]
+                            (fun x0 : environ =>
+                             local
+                               (`(@eq val
+                                    (if @isnil val contents0
+                                     then Vtrue
+                                     else Vfalse)) retval) x0 &&
+                             `(fifo contents0 q0) x0))))
+                     (@PTree.Leaf global_spec))) (@None global_spec)
+               (@PTree.Leaf global_spec)) (@None global_spec)
+            (@PTree.Node global_spec
+               (@PTree.Node global_spec (@PTree.Leaf global_spec)
+                  (@Some global_spec
+                     (Global_func
+                        (WITH _ : unit PRE  [(1%positive, tptr tvoid),
+                         (2%positive, tint)]
+                         PROP  ()
+                         LOCAL ()
+                         SEP 
+                         (`(memory_block Tsh)
+                            (`force_int (eval_id 2%positive))
+                            (eval_id 1%positive)) POST  [tvoid]
+                         (fun _ : environ => @emp mpred Nveric Sveric))))
+                  (@PTree.Node global_spec (@PTree.Leaf global_spec)
+                     (@Some global_spec
+                        (Global_func
+                           (WITH  p0 : val * list val, p : val PRE 
+                            [(_Q, tptr t_struct_fifo)]
+                            (let (q0, contents0) := p0 in
+                             PROP  ()
+                             LOCAL  (`(@eq val q0) (eval_id _Q))
+                             SEP  (`(fifo (p :: contents0) q0))) POST 
+                            [tptr t_struct_elem]
+                            (let (q0, contents0) := p0 in
+                             fun rho : environ =>
+                             local (`(@eq val p) retval) rho &&
+                             `(fifo contents0 q0) rho * `link_ retval rho))))
+                     (@PTree.Leaf global_spec)))
+               (@Some global_spec
+                  (Global_func
+                     (WITH _ : unit PRE  [(1%positive, tdouble)]
+                      (fun _ : environ => !!False) POST  [tdouble]
+                      (fun _ : environ => !!False))))
+               (@PTree.Node global_spec (@PTree.Leaf global_spec)
+                  (@None global_spec)
+                  (@PTree.Node global_spec (@PTree.Leaf global_spec)
+                     (@Some global_spec
+                        (Global_func
+                           (WITH u : unit PRE  []main_pre prog u POST  [tint]
+                            main_post prog u))) (@PTree.Leaf global_spec))))))) in
+PROP  ()
+LOCAL  (tc_environ Delta; `(@eq val hd) (eval_id _h);
+`(@eq val q) (eval_id _Q))
+SEP  (`(field_mapsto Tsh t_struct_fifo _head q hd);
+`(field_mapsto Tsh t_struct_fifo _tail q tl);
+`(if @isnil val contents
+  then !!(hd = nullval) && @emp mpred Nveric Sveric
+  else
+   EX  prefix : list val,
+   !!(contents = prefix ++ tl :: @nil val) &&
+   (@links t_struct_elem _next QS Tsh prefix hd tl * link tl nullval)))
+|-- local
+      (tc_expropt Delta
+         (@Some expr
+            (Ebinop Oeq (Etempvar _h (tptr t_struct_elem))
+               (Ecast (Econst_int (Int.repr 0) tint) (tptr tvoid)) tint))
+         (ret_type Delta)) &&
+    `(function_body_ret_assert tint
+        (local
+           (`(@eq val (if @isnil val contents then Vtrue else Vfalse)) retval) &&
+         `(fifo contents q)) EK_return)
+      (cast_expropt
+         (@Some expr
+            (Ebinop Oeq (Etempvar _h (tptr t_struct_elem))
+               (Ecast (Econst_int (Int.repr 0) tint) (tptr tvoid)) tint))
+         (ret_type Delta)) (@id environ)
+. Proof. intros Q h. ungather_entail.
+entailer.
+unfold fifo.
+normalize.
+apply exp_right with (h,tl).
+apply andp_right; auto.
+destruct (isnil contents).
+* normalize. apply prop_right; subst.
+  simpl. auto.
+* normalize. unfold link.
+ entailer.
+ destruct prefix.
+ + rewrite links_nil_eq.
+    entailer. apply ptr_eq_e in H4; subst.
+    destruct tl; inv H2; simpl; auto.
+ + rewrite links_cons_eq.
+ entailer!.
+ destruct h; inv H6; simpl; auto.
+Qed.
+
+Lemma goal_2 :
+name _Q ->
+name _Q' ->
+EVAR
+  (forall Frame : list (environ -> mpred),
+   let Delta :=
+     @abbreviate tycontext
+       (@PTree.Node (type * bool)
+          (@PTree.Node (type * bool)
+             (@PTree.Node (type * bool)
+                (@PTree.Node (type * bool)
+                   (@PTree.Node (type * bool)
+                      (@PTree.Node (type * bool) (@PTree.Leaf (type * bool))
+                         (@Some (type * bool) (tptr tvoid, false))
+                         (@PTree.Leaf (type * bool))) (@None (type * bool))
+                      (@PTree.Leaf (type * bool))) (@None (type * bool))
+                   (@PTree.Leaf (type * bool))) (@None (type * bool))
+                (@PTree.Leaf (type * bool))) (@None (type * bool))
+             (@PTree.Leaf (type * bool))) (@None (type * bool))
+          (@PTree.Node (type * bool) (@PTree.Leaf (type * bool))
+             (@None (type * bool))
+             (@PTree.Node (type * bool)
+                (@PTree.Node (type * bool)
+                   (@PTree.Node (type * bool) (@PTree.Leaf (type * bool))
+                      (@Some (type * bool) (tptr t_struct_fifo, false))
+                      (@PTree.Leaf (type * bool))) (@None (type * bool))
+                   (@PTree.Leaf (type * bool))) (@None (type * bool))
+                (@PTree.Leaf (type * bool)))), PTree.empty type,
+       tptr t_struct_fifo,
+       @PTree.Node global_spec
+         (@PTree.Node global_spec
+            (@PTree.Node global_spec
+               (@PTree.Node global_spec (@PTree.Leaf global_spec)
+                  (@Some global_spec
+                     (Global_func
+                        (WITH _ : unit PRE  [(1%positive, tptr tvoid),
+                         (2%positive, tptr tvoid), (3%positive, tuint),
+                         (4%positive, tuint)](fun _ : environ => !!False)
+                         POST  [tvoid](fun _ : environ => !!False))))
+                  (@PTree.Node global_spec (@PTree.Leaf global_spec)
+                     (@Some global_spec
+                        (Global_func
+                           (WITH  p0 : val * list val, p : val PRE 
+                            [(_Q, tptr t_struct_fifo),
+                            (_p, tptr t_struct_elem)]
+                            (let (q, contents) := p0 in
+                             PROP  ()
+                             LOCAL  (`(@eq val q) (eval_id _Q);
+                             `(@eq val p) (eval_id _p))
+                             SEP  (`(fifo contents q); `(link_ p))) POST 
+                            [tvoid]
+                            (let (q, contents) := p0 in
+                             `(fifo (contents ++ p :: @nil val) q)))))
+                     (@PTree.Leaf global_spec))) (@None global_spec)
+               (@PTree.Node global_spec
+                  (@PTree.Node global_spec (@PTree.Leaf global_spec)
+                     (@Some global_spec
+                        (Global_func
+                           (WITH _ : unit PRE  []
+                            (fun _ : environ => @emp mpred Nveric Sveric)
+                            POST  [tptr t_struct_fifo]
+                            `(fifo (@nil val)) retval)))
+                     (@PTree.Leaf global_spec)) (@None global_spec)
+                  (@PTree.Node global_spec (@PTree.Leaf global_spec)
+                     (@Some global_spec
+                        (Global_func
+                           (WITH  a : int, b : int PRE  [(_a, tint),
+                            (_b, tint)]
+                            PROP  ()
+                            LOCAL  (`(@eq val (Vint a)) (eval_id _a);
+                            `(@eq val (Vint b)) (eval_id _b))  SEP() POST 
+                            [tptr t_struct_elem]`(elemrep (a, b)) retval)))
+                     (@PTree.Leaf global_spec)))) (@None global_spec)
+            (@PTree.Node global_spec
+               (@PTree.Node global_spec (@PTree.Leaf global_spec)
+                  (@Some global_spec
+                     (Global_func
+                        (WITH n : int PRE  [(1%positive, tint)]
+                         PROP  (4 <= Int.signed n)
+                         LOCAL  (`(@eq val (Vint n)) (eval_id 1%positive))
+                         SEP() POST  [tptr tvoid]`(memory_block Tsh n) retval)))
+                  (@PTree.Leaf global_spec)) (@None global_spec)
+               (@PTree.Leaf global_spec))) (@None global_spec)
+         (@PTree.Node global_spec
+            (@PTree.Node global_spec
+               (@PTree.Node global_spec (@PTree.Leaf global_spec)
+                  (@Some global_spec
+                     (Global_func
+                        (WITH _ : unit PRE  [(1%positive, tptr tschar),
+                         (2%positive, tint)](fun _ : environ => !!False)
+                         POST  [tint](fun _ : environ => !!False))))
+                  (@PTree.Node global_spec (@PTree.Leaf global_spec)
+                     (@Some global_spec
+                        (Global_func
+                           (WITH  q : val, contents : list val PRE 
+                            [(_Q, tptr t_struct_fifo)]
+                            PROP  ()
+                            LOCAL  (`(@eq val q) (eval_id _Q))
+                            SEP  (`(fifo contents q)) POST  [tint]
+                            (fun x0 : environ =>
+                             local
+                               (`(@eq val
+                                    (if @isnil val contents
+                                     then Vtrue
+                                     else Vfalse)) retval) x0 &&
+                             `(fifo contents q) x0))))
+                     (@PTree.Leaf global_spec))) (@None global_spec)
+               (@PTree.Leaf global_spec)) (@None global_spec)
+            (@PTree.Node global_spec
+               (@PTree.Node global_spec (@PTree.Leaf global_spec)
+                  (@Some global_spec
+                     (Global_func
+                        (WITH _ : unit PRE  [(1%positive, tptr tvoid),
+                         (2%positive, tint)]
+                         PROP  ()
+                         LOCAL ()
+                         SEP 
+                         (`(memory_block Tsh)
+                            (`force_int (eval_id 2%positive))
+                            (eval_id 1%positive)) POST  [tvoid]
+                         (fun _ : environ => @emp mpred Nveric Sveric))))
+                  (@PTree.Node global_spec (@PTree.Leaf global_spec)
+                     (@Some global_spec
+                        (Global_func
+                           (WITH  p0 : val * list val, p : val PRE 
+                            [(_Q, tptr t_struct_fifo)]
+                            (let (q, contents) := p0 in
+                             PROP  ()
+                             LOCAL  (`(@eq val q) (eval_id _Q))
+                             SEP  (`(fifo (p :: contents) q))) POST 
+                            [tptr t_struct_elem]
+                            (let (q, contents) := p0 in
+                             fun rho : environ =>
+                             local (`(@eq val p) retval) rho &&
+                             `(fifo contents q) rho * `link_ retval rho))))
+                     (@PTree.Leaf global_spec)))
+               (@Some global_spec
+                  (Global_func
+                     (WITH _ : unit PRE  [(1%positive, tdouble)]
+                      (fun _ : environ => !!False) POST  [tdouble]
+                      (fun _ : environ => !!False))))
+               (@PTree.Node global_spec (@PTree.Leaf global_spec)
+                  (@None global_spec)
+                  (@PTree.Node global_spec (@PTree.Leaf global_spec)
+                     (@Some global_spec
+                        (Global_func
+                           (WITH u : unit PRE  []main_pre prog u POST  [tint]
+                            main_post prog u))) (@PTree.Leaf global_spec)))))) in
+   let witness := Int.repr 8 in
+   PROP  ()  LOCAL  (tc_environ Delta)  SEP()
+   |-- PROP  ()
+       LOCAL 
+       (tc_exprlist Delta
+          (@snd (list ident) (list type)
+             (@split ident type
+                (@fst (list (ident * type)) type
+                   ((1%positive, tint) :: @nil (positive * type), tptr tvoid))))
+          (Econst_int (Int.repr 8) tuint :: @nil expr))
+       (SEPx
+          (`(PROP  (4 <= Int.signed witness)
+             LOCAL  (`(@eq val (Vint witness)) (eval_id 1%positive))  SEP())
+             (make_args'
+                ((1%positive, tint) :: @nil (positive * type), tptr tvoid)
+                (eval_exprlist
+                   (@snd (list ident) (list type)
+                      (@split ident type
+                         (@fst (list (ident * type)) type
+                            ((1%positive, tint) :: @nil (positive * type),
+                            tptr tvoid))))
+                   (Econst_int (Int.repr 8) tuint :: @nil expr))) :: Frame)))
+. Proof. intros Q Q'; ungather_entail.
+entailer!.
+compute; congruence.
+Qed.
+
+Lemma goal_3 :
+name _Q ->
+name _Q' ->
+let Delta :=
+  @abbreviate tycontext
+    (initialized _Q
+       (initialized _Q'
+          (@PTree.Node (type * bool)
+             (@PTree.Node (type * bool)
+                (@PTree.Node (type * bool)
+                   (@PTree.Node (type * bool)
+                      (@PTree.Node (type * bool)
+                         (@PTree.Node (type * bool)
+                            (@PTree.Leaf (type * bool))
+                            (@Some (type * bool) (tptr tvoid, false))
+                            (@PTree.Leaf (type * bool)))
+                         (@None (type * bool)) (@PTree.Leaf (type * bool)))
+                      (@None (type * bool)) (@PTree.Leaf (type * bool)))
+                   (@None (type * bool)) (@PTree.Leaf (type * bool)))
+                (@None (type * bool)) (@PTree.Leaf (type * bool)))
+             (@None (type * bool))
+             (@PTree.Node (type * bool) (@PTree.Leaf (type * bool))
+                (@None (type * bool))
+                (@PTree.Node (type * bool)
+                   (@PTree.Node (type * bool)
+                      (@PTree.Node (type * bool) (@PTree.Leaf (type * bool))
+                         (@Some (type * bool) (tptr t_struct_fifo, false))
+                         (@PTree.Leaf (type * bool))) (@None (type * bool))
+                      (@PTree.Leaf (type * bool))) (@None (type * bool))
+                   (@PTree.Leaf (type * bool)))), PTree.empty type,
+          tptr t_struct_fifo,
+          @PTree.Node global_spec
+            (@PTree.Node global_spec
+               (@PTree.Node global_spec
+                  (@PTree.Node global_spec (@PTree.Leaf global_spec)
+                     (@Some global_spec
+                        (Global_func
+                           (WITH _ : unit PRE  [(1%positive, tptr tvoid),
+                            (2%positive, tptr tvoid), (3%positive, tuint),
+                            (4%positive, tuint)](fun _ : environ => !!False)
+                            POST  [tvoid](fun _ : environ => !!False))))
+                     (@PTree.Node global_spec (@PTree.Leaf global_spec)
+                        (@Some global_spec
+                           (Global_func
+                              (WITH  p0 : val * list val, p : val PRE 
+                               [(_Q, tptr t_struct_fifo),
+                               (_p, tptr t_struct_elem)]
+                               (let (q, contents) := p0 in
+                                PROP  ()
+                                LOCAL  (`(@eq val q) (eval_id _Q);
+                                `(@eq val p) (eval_id _p))
+                                SEP  (`(fifo contents q); `(link_ p))) POST 
+                               [tvoid]
+                               (let (q, contents) := p0 in
+                                `(fifo (contents ++ p :: @nil val) q)))))
+                        (@PTree.Leaf global_spec))) (@None global_spec)
+                  (@PTree.Node global_spec
+                     (@PTree.Node global_spec (@PTree.Leaf global_spec)
+                        (@Some global_spec
+                           (Global_func
+                              (WITH _ : unit PRE  []
+                               (fun _ : environ => @emp mpred Nveric Sveric)
+                               POST  [tptr t_struct_fifo]
+                               `(fifo (@nil val)) retval)))
+                        (@PTree.Leaf global_spec)) (@None global_spec)
+                     (@PTree.Node global_spec (@PTree.Leaf global_spec)
+                        (@Some global_spec
+                           (Global_func
+                              (WITH  a : int, b : int PRE  [(_a, tint),
+                               (_b, tint)]
+                               PROP  ()
+                               LOCAL  (`(@eq val (Vint a)) (eval_id _a);
+                               `(@eq val (Vint b)) (eval_id _b))  SEP() POST 
+                               [tptr t_struct_elem]`(elemrep (a, b)) retval)))
+                        (@PTree.Leaf global_spec)))) (@None global_spec)
+               (@PTree.Node global_spec
+                  (@PTree.Node global_spec (@PTree.Leaf global_spec)
+                     (@Some global_spec
+                        (Global_func
+                           (WITH n : int PRE  [(1%positive, tint)]
+                            PROP  (4 <= Int.signed n)
+                            LOCAL  (`(@eq val (Vint n)) (eval_id 1%positive))
+                              SEP() POST  [tptr tvoid]
+                            `(memory_block Tsh n) retval)))
+                     (@PTree.Leaf global_spec)) (@None global_spec)
+                  (@PTree.Leaf global_spec))) (@None global_spec)
+            (@PTree.Node global_spec
+               (@PTree.Node global_spec
+                  (@PTree.Node global_spec (@PTree.Leaf global_spec)
+                     (@Some global_spec
+                        (Global_func
+                           (WITH _ : unit PRE  [(1%positive, tptr tschar),
+                            (2%positive, tint)](fun _ : environ => !!False)
+                            POST  [tint](fun _ : environ => !!False))))
+                     (@PTree.Node global_spec (@PTree.Leaf global_spec)
+                        (@Some global_spec
+                           (Global_func
+                              (WITH  q : val, contents : list val PRE 
+                               [(_Q, tptr t_struct_fifo)]
+                               PROP  ()
+                               LOCAL  (`(@eq val q) (eval_id _Q))
+                               SEP  (`(fifo contents q)) POST  [tint]
+                               (fun x0 : environ =>
+                                local
+                                  (`(@eq val
+                                       (if @isnil val contents
+                                        then Vtrue
+                                        else Vfalse)) retval) x0 &&
+                                `(fifo contents q) x0))))
+                        (@PTree.Leaf global_spec))) (@None global_spec)
+                  (@PTree.Leaf global_spec)) (@None global_spec)
+               (@PTree.Node global_spec
+                  (@PTree.Node global_spec (@PTree.Leaf global_spec)
+                     (@Some global_spec
+                        (Global_func
+                           (WITH _ : unit PRE  [(1%positive, tptr tvoid),
+                            (2%positive, tint)]
+                            PROP  ()
+                            LOCAL ()
+                            SEP 
+                            (`(memory_block Tsh)
+                               (`force_int (eval_id 2%positive))
+                               (eval_id 1%positive)) POST  [tvoid]
+                            (fun _ : environ => @emp mpred Nveric Sveric))))
+                     (@PTree.Node global_spec (@PTree.Leaf global_spec)
+                        (@Some global_spec
+                           (Global_func
+                              (WITH  p0 : val * list val, p : val PRE 
+                               [(_Q, tptr t_struct_fifo)]
+                               (let (q, contents) := p0 in
+                                PROP  ()
+                                LOCAL  (`(@eq val q) (eval_id _Q))
+                                SEP  (`(fifo (p :: contents) q))) POST 
+                               [tptr t_struct_elem]
+                               (let (q, contents) := p0 in
+                                fun rho : environ =>
+                                local (`(@eq val p) retval) rho &&
+                                `(fifo contents q) rho * `link_ retval rho))))
+                        (@PTree.Leaf global_spec)))
+                  (@Some global_spec
+                     (Global_func
+                        (WITH _ : unit PRE  [(1%positive, tdouble)]
+                         (fun _ : environ => !!False) POST  [tdouble]
+                         (fun _ : environ => !!False))))
+                  (@PTree.Node global_spec (@PTree.Leaf global_spec)
+                     (@None global_spec)
+                     (@PTree.Node global_spec (@PTree.Leaf global_spec)
+                        (@Some global_spec
+                           (Global_func
+                              (WITH u : unit PRE  []main_pre prog u POST 
+                               [tint]main_post prog u)))
+                        (@PTree.Leaf global_spec)))))))) in
+PROP  ()
+LOCAL  (tc_environ Delta;
+`(@eq val) (eval_id _Q)
+  (eval_expr (Ecast (Etempvar _Q' (tptr tvoid)) (tptr t_struct_fifo))))
+SEP  (`(memory_block Tsh (Int.repr 8)) (eval_id _Q'))
+|-- PROP  ()  LOCAL ()  SEP  (`(memory_block Tsh (Int.repr 8)) (eval_id _Q))
+. Proof. intros Q Q'; ungather_entail.
+entailer.
+Qed.
+
+Lemma goal_4 :
+name _Q ->
+name _Q' ->
+EVAR
+  (forall n : nat,
+   EVAR
+     (forall sh : share,
+      let Delta :=
+        @abbreviate tycontext
+          (initialized _Q
+             (initialized _Q'
+                (@PTree.Node (type * bool)
+                   (@PTree.Node (type * bool)
+                      (@PTree.Node (type * bool)
+                         (@PTree.Node (type * bool)
+                            (@PTree.Node (type * bool)
+                               (@PTree.Node (type * bool)
+                                  (@PTree.Leaf (type * bool))
+                                  (@Some (type * bool) (tptr tvoid, false))
+                                  (@PTree.Leaf (type * bool)))
+                               (@None (type * bool))
+                               (@PTree.Leaf (type * bool)))
+                            (@None (type * bool)) (@PTree.Leaf (type * bool)))
+                         (@None (type * bool)) (@PTree.Leaf (type * bool)))
+                      (@None (type * bool)) (@PTree.Leaf (type * bool)))
+                   (@None (type * bool))
+                   (@PTree.Node (type * bool) (@PTree.Leaf (type * bool))
+                      (@None (type * bool))
+                      (@PTree.Node (type * bool)
+                         (@PTree.Node (type * bool)
+                            (@PTree.Node (type * bool)
+                               (@PTree.Leaf (type * bool))
+                               (@Some (type * bool)
+                                  (tptr t_struct_fifo, false))
+                               (@PTree.Leaf (type * bool)))
+                            (@None (type * bool)) (@PTree.Leaf (type * bool)))
+                         (@None (type * bool)) (@PTree.Leaf (type * bool)))),
+                PTree.empty type, tptr t_struct_fifo,
+                @PTree.Node global_spec
+                  (@PTree.Node global_spec
+                     (@PTree.Node global_spec
+                        (@PTree.Node global_spec (@PTree.Leaf global_spec)
+                           (@Some global_spec
+                              (Global_func
+                                 (WITH _ : unit PRE 
+                                  [(1%positive, tptr tvoid),
+                                  (2%positive, tptr tvoid),
+                                  (3%positive, tuint), (4%positive, tuint)]
+                                  (fun _ : environ => !!False) POST  [tvoid]
+                                  (fun _ : environ => !!False))))
+                           (@PTree.Node global_spec (@PTree.Leaf global_spec)
+                              (@Some global_spec
+                                 (Global_func
+                                    (WITH  p0 : val * list val, p : val PRE 
+                                     [(_Q, tptr t_struct_fifo),
+                                     (_p, tptr t_struct_elem)]
+                                     (let (q, contents) := p0 in
+                                      PROP  ()
+                                      LOCAL  (`(@eq val q) (eval_id _Q);
+                                      `(@eq val p) (eval_id _p))
+                                      SEP  (`(fifo contents q); `(link_ p)))
+                                     POST  [tvoid]
+                                     (let (q, contents) := p0 in
+                                      `(fifo (contents ++ p :: @nil val) q)))))
+                              (@PTree.Leaf global_spec))) (@None global_spec)
+                        (@PTree.Node global_spec
+                           (@PTree.Node global_spec (@PTree.Leaf global_spec)
+                              (@Some global_spec
+                                 (Global_func
+                                    (WITH _ : unit PRE  []
+                                     (fun _ : environ =>
+                                      @emp mpred Nveric Sveric) POST 
+                                     [tptr t_struct_fifo]
+                                     `(fifo (@nil val)) retval)))
+                              (@PTree.Leaf global_spec)) (@None global_spec)
+                           (@PTree.Node global_spec (@PTree.Leaf global_spec)
+                              (@Some global_spec
+                                 (Global_func
+                                    (WITH  a : int, b : int PRE  [(_a, tint),
+                                     (_b, tint)]
+                                     PROP  ()
+                                     LOCAL 
+                                     (`(@eq val (Vint a)) (eval_id _a);
+                                     `(@eq val (Vint b)) (eval_id _b))  
+                                     SEP() POST  [tptr t_struct_elem]
+                                     `(elemrep (a, b)) retval)))
+                              (@PTree.Leaf global_spec))))
+                     (@None global_spec)
+                     (@PTree.Node global_spec
+                        (@PTree.Node global_spec (@PTree.Leaf global_spec)
+                           (@Some global_spec
+                              (Global_func
+                                 (WITH n0 : int PRE  [(1%positive, tint)]
+                                  PROP  (4 <= Int.signed n0)
+                                  LOCAL 
+                                  (`(@eq val (Vint n0)) (eval_id 1%positive))
+                                    SEP() POST  [tptr tvoid]
+                                  `(memory_block Tsh n0) retval)))
+                           (@PTree.Leaf global_spec)) (@None global_spec)
+                        (@PTree.Leaf global_spec))) (@None global_spec)
+                  (@PTree.Node global_spec
+                     (@PTree.Node global_spec
+                        (@PTree.Node global_spec (@PTree.Leaf global_spec)
+                           (@Some global_spec
+                              (Global_func
+                                 (WITH _ : unit PRE 
+                                  [(1%positive, tptr tschar),
+                                  (2%positive, tint)]
+                                  (fun _ : environ => !!False) POST  [tint]
+                                  (fun _ : environ => !!False))))
+                           (@PTree.Node global_spec (@PTree.Leaf global_spec)
+                              (@Some global_spec
+                                 (Global_func
+                                    (WITH  q : val, contents : list val PRE 
+                                     [(_Q, tptr t_struct_fifo)]
+                                     PROP  ()
+                                     LOCAL  (`(@eq val q) (eval_id _Q))
+                                     SEP  (`(fifo contents q)) POST  [tint]
+                                     (fun x0 : environ =>
+                                      local
+                                        (`(@eq val
+                                             (if @isnil val contents
+                                              then Vtrue
+                                              else Vfalse)) retval) x0 &&
+                                      `(fifo contents q) x0))))
+                              (@PTree.Leaf global_spec))) (@None global_spec)
+                        (@PTree.Leaf global_spec)) (@None global_spec)
+                     (@PTree.Node global_spec
+                        (@PTree.Node global_spec (@PTree.Leaf global_spec)
+                           (@Some global_spec
+                              (Global_func
+                                 (WITH _ : unit PRE 
+                                  [(1%positive, tptr tvoid),
+                                  (2%positive, tint)]
+                                  PROP  ()
+                                  LOCAL ()
+                                  SEP 
+                                  (`(memory_block Tsh)
+                                     (`force_int (eval_id 2%positive))
+                                     (eval_id 1%positive)) POST  [tvoid]
+                                  (fun _ : environ =>
+                                   @emp mpred Nveric Sveric))))
+                           (@PTree.Node global_spec (@PTree.Leaf global_spec)
+                              (@Some global_spec
+                                 (Global_func
+                                    (WITH  p0 : val * list val, p : val PRE 
+                                     [(_Q, tptr t_struct_fifo)]
+                                     (let (q, contents) := p0 in
+                                      PROP  ()
+                                      LOCAL  (`(@eq val q) (eval_id _Q))
+                                      SEP  (`(fifo (p :: contents) q))) POST 
+                                     [tptr t_struct_elem]
+                                     (let (q, contents) := p0 in
+                                      fun rho : environ =>
+                                      local (`(@eq val p) retval) rho &&
+                                      `(fifo contents q) rho *
+                                      `link_ retval rho))))
+                              (@PTree.Leaf global_spec)))
+                        (@Some global_spec
+                           (Global_func
+                              (WITH _ : unit PRE  [(1%positive, tdouble)]
+                               (fun _ : environ => !!False) POST  [tdouble]
+                               (fun _ : environ => !!False))))
+                        (@PTree.Node global_spec (@PTree.Leaf global_spec)
+                           (@None global_spec)
+                           (@PTree.Node global_spec (@PTree.Leaf global_spec)
+                              (@Some global_spec
+                                 (Global_func
+                                    (WITH u : unit PRE  []main_pre prog u
+                                     POST  [tint]main_post prog u)))
+                              (@PTree.Leaf global_spec)))))))) in
+      PROP  ()
+      LOCAL  (tc_environ Delta)
+      SEP 
+      (`(@numbd (lift_T (Tarrow val (Tarrow val (LiftEnviron mpred)))) 0
+           (field_mapsto Tsh
+              (Tstruct _struct_fifo
+                 (Fcons _head
+                    (tptr
+                       (Tstruct _struct_elem
+                          (Fcons _a tint
+                             (Fcons _b tint
+                                (Fcons _next (Tcomp_ptr _struct_elem noattr)
+                                   Fnil))) noattr))
+                    (Fcons _tail
+                       (tptr
+                          (Tstruct _struct_elem
+                             (Fcons _a tint
+                                (Fcons _b tint
+                                   (Fcons _next
+                                      (Tcomp_ptr _struct_elem noattr) Fnil)))
+                             noattr)) Fnil)) noattr) _head))
+         (eval_lvalue
+            (Ederef (Etempvar _Q (tptr t_struct_fifo)) t_struct_fifo))
+         (`(eval_cast
+              (typeof (Ecast (Econst_int (Int.repr 0) tint) (tptr tvoid)))
+              (tptr t_struct_elem))
+            (eval_expr (Ecast (Econst_int (Int.repr 0) tint) (tptr tvoid))));
+      `(@numbd (lift_T (Tarrow val (LiftEnviron mpred))) 1
+          (field_mapsto_ Tsh t_struct_fifo _tail)) (eval_id _Q))
+      |-- `(@numbd (val -> mpred) n
+              (field_mapsto_ sh
+                 (typeof
+                    (Ederef (Etempvar _Q (tptr t_struct_fifo)) t_struct_fifo))
+                 _tail))
+            (eval_lvalue
+               (Ederef (Etempvar _Q (tptr t_struct_fifo)) t_struct_fifo)) *
+          @TT (LiftEnviron mpred) (@LiftNatDed' mpred Nveric)))
+. Proof. intros Q Q'; ungather_entail.
+unfold sh,n; entailer; cancel.
+Qed.
+
+Lemma goal_5 :
+name _Q ->
+name _Q' ->
+let Delta :=
+  @abbreviate tycontext
+    (initialized _Q
+       (initialized _Q'
+          (@PTree.Node (type * bool)
+             (@PTree.Node (type * bool)
+                (@PTree.Node (type * bool)
+                   (@PTree.Node (type * bool)
+                      (@PTree.Node (type * bool)
+                         (@PTree.Node (type * bool)
+                            (@PTree.Leaf (type * bool))
+                            (@Some (type * bool) (tptr tvoid, false))
+                            (@PTree.Leaf (type * bool)))
+                         (@None (type * bool)) (@PTree.Leaf (type * bool)))
+                      (@None (type * bool)) (@PTree.Leaf (type * bool)))
+                   (@None (type * bool)) (@PTree.Leaf (type * bool)))
+                (@None (type * bool)) (@PTree.Leaf (type * bool)))
+             (@None (type * bool))
+             (@PTree.Node (type * bool) (@PTree.Leaf (type * bool))
+                (@None (type * bool))
+                (@PTree.Node (type * bool)
+                   (@PTree.Node (type * bool)
+                      (@PTree.Node (type * bool) (@PTree.Leaf (type * bool))
+                         (@Some (type * bool) (tptr t_struct_fifo, false))
+                         (@PTree.Leaf (type * bool))) (@None (type * bool))
+                      (@PTree.Leaf (type * bool))) (@None (type * bool))
+                   (@PTree.Leaf (type * bool)))), PTree.empty type,
+          tptr t_struct_fifo,
+          @PTree.Node global_spec
+            (@PTree.Node global_spec
+               (@PTree.Node global_spec
+                  (@PTree.Node global_spec (@PTree.Leaf global_spec)
+                     (@Some global_spec
+                        (Global_func
+                           (WITH _ : unit PRE  [(1%positive, tptr tvoid),
+                            (2%positive, tptr tvoid), (3%positive, tuint),
+                            (4%positive, tuint)](fun _ : environ => !!False)
+                            POST  [tvoid](fun _ : environ => !!False))))
+                     (@PTree.Node global_spec (@PTree.Leaf global_spec)
+                        (@Some global_spec
+                           (Global_func
+                              (WITH  p0 : val * list val, p : val PRE 
+                               [(_Q, tptr t_struct_fifo),
+                               (_p, tptr t_struct_elem)]
+                               (let (q, contents) := p0 in
+                                PROP  ()
+                                LOCAL  (`(@eq val q) (eval_id _Q);
+                                `(@eq val p) (eval_id _p))
+                                SEP  (`(fifo contents q); `(link_ p))) POST 
+                               [tvoid]
+                               (let (q, contents) := p0 in
+                                `(fifo (contents ++ p :: @nil val) q)))))
+                        (@PTree.Leaf global_spec))) (@None global_spec)
+                  (@PTree.Node global_spec
+                     (@PTree.Node global_spec (@PTree.Leaf global_spec)
+                        (@Some global_spec
+                           (Global_func
+                              (WITH _ : unit PRE  []
+                               (fun _ : environ => @emp mpred Nveric Sveric)
+                               POST  [tptr t_struct_fifo]
+                               `(fifo (@nil val)) retval)))
+                        (@PTree.Leaf global_spec)) (@None global_spec)
+                     (@PTree.Node global_spec (@PTree.Leaf global_spec)
+                        (@Some global_spec
+                           (Global_func
+                              (WITH  a : int, b : int PRE  [(_a, tint),
+                               (_b, tint)]
+                               PROP  ()
+                               LOCAL  (`(@eq val (Vint a)) (eval_id _a);
+                               `(@eq val (Vint b)) (eval_id _b))  SEP() POST 
+                               [tptr t_struct_elem]`(elemrep (a, b)) retval)))
+                        (@PTree.Leaf global_spec)))) (@None global_spec)
+               (@PTree.Node global_spec
+                  (@PTree.Node global_spec (@PTree.Leaf global_spec)
+                     (@Some global_spec
+                        (Global_func
+                           (WITH n : int PRE  [(1%positive, tint)]
+                            PROP  (4 <= Int.signed n)
+                            LOCAL  (`(@eq val (Vint n)) (eval_id 1%positive))
+                              SEP() POST  [tptr tvoid]
+                            `(memory_block Tsh n) retval)))
+                     (@PTree.Leaf global_spec)) (@None global_spec)
+                  (@PTree.Leaf global_spec))) (@None global_spec)
+            (@PTree.Node global_spec
+               (@PTree.Node global_spec
+                  (@PTree.Node global_spec (@PTree.Leaf global_spec)
+                     (@Some global_spec
+                        (Global_func
+                           (WITH _ : unit PRE  [(1%positive, tptr tschar),
+                            (2%positive, tint)](fun _ : environ => !!False)
+                            POST  [tint](fun _ : environ => !!False))))
+                     (@PTree.Node global_spec (@PTree.Leaf global_spec)
+                        (@Some global_spec
+                           (Global_func
+                              (WITH  q : val, contents : list val PRE 
+                               [(_Q, tptr t_struct_fifo)]
+                               PROP  ()
+                               LOCAL  (`(@eq val q) (eval_id _Q))
+                               SEP  (`(fifo contents q)) POST  [tint]
+                               (fun x0 : environ =>
+                                local
+                                  (`(@eq val
+                                       (if @isnil val contents
+                                        then Vtrue
+                                        else Vfalse)) retval) x0 &&
+                                `(fifo contents q) x0))))
+                        (@PTree.Leaf global_spec))) (@None global_spec)
+                  (@PTree.Leaf global_spec)) (@None global_spec)
+               (@PTree.Node global_spec
+                  (@PTree.Node global_spec (@PTree.Leaf global_spec)
+                     (@Some global_spec
+                        (Global_func
+                           (WITH _ : unit PRE  [(1%positive, tptr tvoid),
+                            (2%positive, tint)]
+                            PROP  ()
+                            LOCAL ()
+                            SEP 
+                            (`(memory_block Tsh)
+                               (`force_int (eval_id 2%positive))
+                               (eval_id 1%positive)) POST  [tvoid]
+                            (fun _ : environ => @emp mpred Nveric Sveric))))
+                     (@PTree.Node global_spec (@PTree.Leaf global_spec)
+                        (@Some global_spec
+                           (Global_func
+                              (WITH  p0 : val * list val, p : val PRE 
+                               [(_Q, tptr t_struct_fifo)]
+                               (let (q, contents) := p0 in
+                                PROP  ()
+                                LOCAL  (`(@eq val q) (eval_id _Q))
+                                SEP  (`(fifo (p :: contents) q))) POST 
+                               [tptr t_struct_elem]
+                               (let (q, contents) := p0 in
+                                fun rho : environ =>
+                                local (`(@eq val p) retval) rho &&
+                                `(fifo contents q) rho * `link_ retval rho))))
+                        (@PTree.Leaf global_spec)))
+                  (@Some global_spec
+                     (Global_func
+                        (WITH _ : unit PRE  [(1%positive, tdouble)]
+                         (fun _ : environ => !!False) POST  [tdouble]
+                         (fun _ : environ => !!False))))
+                  (@PTree.Node global_spec (@PTree.Leaf global_spec)
+                     (@None global_spec)
+                     (@PTree.Node global_spec (@PTree.Leaf global_spec)
+                        (@Some global_spec
+                           (Global_func
+                              (WITH u : unit PRE  []main_pre prog u POST 
+                               [tint]main_post prog u)))
+                        (@PTree.Leaf global_spec)))))))) in
+PROP  ()
+LOCAL  (tc_environ Delta)
+SEP 
+(`(field_mapsto Tsh
+     (Tstruct _struct_fifo
+        (Fcons _head
+           (tptr
+              (Tstruct _struct_elem
+                 (Fcons _a tint
+                    (Fcons _b tint
+                       (Fcons _next (Tcomp_ptr _struct_elem noattr) Fnil)))
+                 noattr))
+           (Fcons _tail
+              (tptr
+                 (Tstruct _struct_elem
+                    (Fcons _a tint
+                       (Fcons _b tint
+                          (Fcons _next (Tcomp_ptr _struct_elem noattr) Fnil)))
+                    noattr)) Fnil)) noattr) _head)
+   (eval_lvalue (Ederef (Etempvar _Q (tptr t_struct_fifo)) t_struct_fifo))
+   (`(eval_cast (typeof (Ecast (Econst_int (Int.repr 0) tint) (tptr tvoid)))
+        (tptr t_struct_elem))
+      (eval_expr (Ecast (Econst_int (Int.repr 0) tint) (tptr tvoid))));
+`(field_mapsto Tsh
+    (Tstruct _struct_fifo
+       (Fcons _head
+          (tptr
+             (Tstruct _struct_elem
+                (Fcons _a tint
+                   (Fcons _b tint
+                      (Fcons _next (Tcomp_ptr _struct_elem noattr) Fnil)))
+                noattr))
+          (Fcons _tail
+             (tptr
+                (Tstruct _struct_elem
+                   (Fcons _a tint
+                      (Fcons _b tint
+                         (Fcons _next (Tcomp_ptr _struct_elem noattr) Fnil)))
+                   noattr)) Fnil)) noattr) _tail)
+  (eval_lvalue (Ederef (Etempvar _Q (tptr t_struct_fifo)) t_struct_fifo))
+  (`(eval_cast (typeof (Ecast (Econst_int (Int.repr 0) tint) (tptr tvoid)))
+       (tptr t_struct_elem))
+     (eval_expr (Ecast (Econst_int (Int.repr 0) tint) (tptr tvoid)))))
+|-- local
+      (tc_expropt Delta (@Some expr (Etempvar _Q (tptr t_struct_fifo)))
+         (ret_type Delta)) &&
+    `(function_body_ret_assert (tptr t_struct_fifo)
+        (`(fifo (@nil val)) retval) EK_return)
+      (cast_expropt (@Some expr (Etempvar _Q (tptr t_struct_fifo)))
+         (ret_type Delta)) (@id environ)
+. Proof. intros Q Q'; ungather_entail.
+entailer.
+  unfold fifo.
+  apply exp_right with (nullval,nullval).
+   destruct (@isnil val nil); [ | congruence].
+ entailer.
+Qed.
+
+Lemma goal_6 :
+name _Q ->
+name _p ->
+name _h ->
+name _t ->
+forall q p : val,
+let Delta :=
+  @abbreviate tycontext
+    (@PTree.Node (type * bool)
+       (@PTree.Node (type * bool) (@PTree.Leaf (type * bool))
+          (@None (type * bool))
+          (@PTree.Node (type * bool) (@PTree.Leaf (type * bool))
+             (@None (type * bool))
+             (@PTree.Node (type * bool)
+                (@PTree.Node (type * bool) (@PTree.Leaf (type * bool))
+                   (@Some (type * bool) (tptr t_struct_elem, false))
+                   (@PTree.Leaf (type * bool))) (@None (type * bool))
+                (@PTree.Leaf (type * bool))))) (@None (type * bool))
+       (@PTree.Node (type * bool)
+          (@PTree.Node (type * bool) (@PTree.Leaf (type * bool))
+             (@None (type * bool))
+             (@PTree.Node (type * bool)
+                (@PTree.Node (type * bool) (@PTree.Leaf (type * bool))
+                   (@Some (type * bool) (tptr t_struct_elem, true))
+                   (@PTree.Leaf (type * bool))) (@None (type * bool))
+                (@PTree.Leaf (type * bool)))) (@None (type * bool))
+          (@PTree.Node (type * bool)
+             (@PTree.Node (type * bool)
+                (@PTree.Node (type * bool) (@PTree.Leaf (type * bool))
+                   (@Some (type * bool) (tptr t_struct_fifo, true))
+                   (@PTree.Leaf (type * bool))) (@None (type * bool))
+                (@PTree.Leaf (type * bool))) (@None (type * bool))
+             (@PTree.Node (type * bool)
+                (@PTree.Node (type * bool) (@PTree.Leaf (type * bool))
+                   (@Some (type * bool) (tptr t_struct_elem, false))
+                   (@PTree.Leaf (type * bool))) (@None (type * bool))
+                (@PTree.Leaf (type * bool))))), PTree.empty type, tvoid,
+    @PTree.Node global_spec
+      (@PTree.Node global_spec
+         (@PTree.Node global_spec
+            (@PTree.Node global_spec (@PTree.Leaf global_spec)
+               (@Some global_spec
+                  (Global_func
+                     (WITH _ : unit PRE  [(1%positive, tptr tvoid),
+                      (2%positive, tptr tvoid), (3%positive, tuint),
+                      (4%positive, tuint)](fun _ : environ => !!False) POST 
+                      [tvoid](fun _ : environ => !!False))))
+               (@PTree.Node global_spec (@PTree.Leaf global_spec)
+                  (@Some global_spec
+                     (Global_func
+                        (WITH  p0 : val * list val, p1 : val PRE 
+                         [(_Q, tptr t_struct_fifo), (_p, tptr t_struct_elem)]
+                         (let (q0, contents) := p0 in
+                          PROP  ()
+                          LOCAL  (`(@eq val q0) (eval_id _Q);
+                          `(@eq val p1) (eval_id _p))
+                          SEP  (`(fifo contents q0); `(link_ p1))) POST 
+                         [tvoid]
+                         (let (q0, contents) := p0 in
+                          `(fifo (contents ++ p1 :: @nil val) q0)))))
+                  (@PTree.Leaf global_spec))) (@None global_spec)
+            (@PTree.Node global_spec
+               (@PTree.Node global_spec (@PTree.Leaf global_spec)
+                  (@Some global_spec
+                     (Global_func
+                        (WITH _ : unit PRE  []
+                         (fun _ : environ => @emp mpred Nveric Sveric) POST 
+                         [tptr t_struct_fifo]`(fifo (@nil val)) retval)))
+                  (@PTree.Leaf global_spec)) (@None global_spec)
+               (@PTree.Node global_spec (@PTree.Leaf global_spec)
+                  (@Some global_spec
+                     (Global_func
+                        (WITH  a : int, b : int PRE  [(_a, tint), (_b, tint)]
+                         PROP  ()
+                         LOCAL  (`(@eq val (Vint a)) (eval_id _a);
+                         `(@eq val (Vint b)) (eval_id _b))  SEP() POST 
+                         [tptr t_struct_elem]`(elemrep (a, b)) retval)))
+                  (@PTree.Leaf global_spec)))) (@None global_spec)
+         (@PTree.Node global_spec
+            (@PTree.Node global_spec (@PTree.Leaf global_spec)
+               (@Some global_spec
+                  (Global_func
+                     (WITH n : int PRE  [(1%positive, tint)]
+                      PROP  (4 <= Int.signed n)
+                      LOCAL  (`(@eq val (Vint n)) (eval_id 1%positive))
+                      SEP() POST  [tptr tvoid]`(memory_block Tsh n) retval)))
+               (@PTree.Leaf global_spec)) (@None global_spec)
+            (@PTree.Leaf global_spec))) (@None global_spec)
+      (@PTree.Node global_spec
+         (@PTree.Node global_spec
+            (@PTree.Node global_spec (@PTree.Leaf global_spec)
+               (@Some global_spec
+                  (Global_func
+                     (WITH _ : unit PRE  [(1%positive, tptr tschar),
+                      (2%positive, tint)](fun _ : environ => !!False) POST 
+                      [tint](fun _ : environ => !!False))))
+               (@PTree.Node global_spec (@PTree.Leaf global_spec)
+                  (@Some global_spec
+                     (Global_func
+                        (WITH  q0 : val, contents : list val PRE 
+                         [(_Q, tptr t_struct_fifo)]
+                         PROP  ()
+                         LOCAL  (`(@eq val q0) (eval_id _Q))
+                         SEP  (`(fifo contents q0)) POST  [tint]
+                         (fun x0 : environ =>
+                          local
+                            (`(@eq val
+                                 (if @isnil val contents
+                                  then Vtrue
+                                  else Vfalse)) retval) x0 &&
+                          `(fifo contents q0) x0))))
+                  (@PTree.Leaf global_spec))) (@None global_spec)
+            (@PTree.Leaf global_spec)) (@None global_spec)
+         (@PTree.Node global_spec
+            (@PTree.Node global_spec (@PTree.Leaf global_spec)
+               (@Some global_spec
+                  (Global_func
+                     (WITH _ : unit PRE  [(1%positive, tptr tvoid),
+                      (2%positive, tint)]
+                      PROP  ()
+                      LOCAL ()
+                      SEP 
+                      (`(memory_block Tsh) (`force_int (eval_id 2%positive))
+                         (eval_id 1%positive)) POST  [tvoid]
+                      (fun _ : environ => @emp mpred Nveric Sveric))))
+               (@PTree.Node global_spec (@PTree.Leaf global_spec)
+                  (@Some global_spec
+                     (Global_func
+                        (WITH  p0 : val * list val, p1 : val PRE 
+                         [(_Q, tptr t_struct_fifo)]
+                         (let (q0, contents) := p0 in
+                          PROP  ()
+                          LOCAL  (`(@eq val q0) (eval_id _Q))
+                          SEP  (`(fifo (p1 :: contents) q0))) POST 
+                         [tptr t_struct_elem]
+                         (let (q0, contents) := p0 in
+                          fun rho : environ =>
+                          local (`(@eq val p1) retval) rho &&
+                          `(fifo contents q0) rho * `link_ retval rho))))
+                  (@PTree.Leaf global_spec)))
+            (@Some global_spec
+               (Global_func
+                  (WITH _ : unit PRE  [(1%positive, tdouble)]
+                   (fun _ : environ => !!False) POST  [tdouble]
+                   (fun _ : environ => !!False))))
+            (@PTree.Node global_spec (@PTree.Leaf global_spec)
+               (@None global_spec)
+               (@PTree.Node global_spec (@PTree.Leaf global_spec)
+                  (@Some global_spec
+                     (Global_func
+                        (WITH u : unit PRE  []main_pre prog u POST  [tint]
+                         main_post prog u))) (@PTree.Leaf global_spec)))))) in
+PROP  ()
+LOCAL  (tc_environ Delta; `(@eq val q) (eval_id _Q);
+`(@eq val p) (eval_id _p))  SEP  (`(link_ p)) |-- `link_ (eval_id _p)
+. Proof. intros Q p h t; ungather_entail.
+entailer.
+Qed.
+
+Lemma goal_7 :
+name _Q ->
+name _p ->
+name _h ->
+name _t ->
+EVAR
+  (forall n : nat,
+   EVAR
+     (forall (sh : share) (q : val) (contents : list val) (p hd tl : val),
+      let Delta :=
+        @abbreviate tycontext
+          (@PTree.Node (type * bool)
+             (@PTree.Node (type * bool) (@PTree.Leaf (type * bool))
+                (@None (type * bool))
+                (@PTree.Node (type * bool) (@PTree.Leaf (type * bool))
+                   (@None (type * bool))
+                   (@PTree.Node (type * bool)
+                      (@PTree.Node (type * bool) (@PTree.Leaf (type * bool))
+                         (@Some (type * bool) (tptr t_struct_elem, false))
+                         (@PTree.Leaf (type * bool))) (@None (type * bool))
+                      (@PTree.Leaf (type * bool))))) (@None (type * bool))
+             (@PTree.Node (type * bool)
+                (@PTree.Node (type * bool) (@PTree.Leaf (type * bool))
+                   (@None (type * bool))
+                   (@PTree.Node (type * bool)
+                      (@PTree.Node (type * bool) (@PTree.Leaf (type * bool))
+                         (@Some (type * bool) (tptr t_struct_elem, true))
+                         (@PTree.Leaf (type * bool))) (@None (type * bool))
+                      (@PTree.Leaf (type * bool)))) (@None (type * bool))
+                (@PTree.Node (type * bool)
+                   (@PTree.Node (type * bool)
+                      (@PTree.Node (type * bool) (@PTree.Leaf (type * bool))
+                         (@Some (type * bool) (tptr t_struct_fifo, true))
+                         (@PTree.Leaf (type * bool))) (@None (type * bool))
+                      (@PTree.Leaf (type * bool))) (@None (type * bool))
+                   (@PTree.Node (type * bool)
+                      (@PTree.Node (type * bool) (@PTree.Leaf (type * bool))
+                         (@Some (type * bool) (tptr t_struct_elem, false))
+                         (@PTree.Leaf (type * bool))) (@None (type * bool))
+                      (@PTree.Leaf (type * bool))))), PTree.empty type,
+          tvoid,
+          @PTree.Node global_spec
+            (@PTree.Node global_spec
+               (@PTree.Node global_spec
+                  (@PTree.Node global_spec (@PTree.Leaf global_spec)
+                     (@Some global_spec
+                        (Global_func
+                           (WITH _ : unit PRE  [(1%positive, tptr tvoid),
+                            (2%positive, tptr tvoid), (3%positive, tuint),
+                            (4%positive, tuint)](fun _ : environ => !!False)
+                            POST  [tvoid](fun _ : environ => !!False))))
+                     (@PTree.Node global_spec (@PTree.Leaf global_spec)
+                        (@Some global_spec
+                           (Global_func
+                              (WITH  p0 : val * list val, p1 : val PRE 
+                               [(_Q, tptr t_struct_fifo),
+                               (_p, tptr t_struct_elem)]
+                               (let (q0, contents0) := p0 in
+                                PROP  ()
+                                LOCAL  (`(@eq val q0) (eval_id _Q);
+                                `(@eq val p1) (eval_id _p))
+                                SEP  (`(fifo contents0 q0); `(link_ p1)))
+                               POST  [tvoid]
+                               (let (q0, contents0) := p0 in
+                                `(fifo (contents0 ++ p1 :: @nil val) q0)))))
+                        (@PTree.Leaf global_spec))) (@None global_spec)
+                  (@PTree.Node global_spec
+                     (@PTree.Node global_spec (@PTree.Leaf global_spec)
+                        (@Some global_spec
+                           (Global_func
+                              (WITH _ : unit PRE  []
+                               (fun _ : environ => @emp mpred Nveric Sveric)
+                               POST  [tptr t_struct_fifo]
+                               `(fifo (@nil val)) retval)))
+                        (@PTree.Leaf global_spec)) (@None global_spec)
+                     (@PTree.Node global_spec (@PTree.Leaf global_spec)
+                        (@Some global_spec
+                           (Global_func
+                              (WITH  a : int, b : int PRE  [(_a, tint),
+                               (_b, tint)]
+                               PROP  ()
+                               LOCAL  (`(@eq val (Vint a)) (eval_id _a);
+                               `(@eq val (Vint b)) (eval_id _b))  SEP() POST 
+                               [tptr t_struct_elem]`(elemrep (a, b)) retval)))
+                        (@PTree.Leaf global_spec)))) (@None global_spec)
+               (@PTree.Node global_spec
+                  (@PTree.Node global_spec (@PTree.Leaf global_spec)
+                     (@Some global_spec
+                        (Global_func
+                           (WITH n0 : int PRE  [(1%positive, tint)]
+                            PROP  (4 <= Int.signed n0)
+                            LOCAL 
+                            (`(@eq val (Vint n0)) (eval_id 1%positive))
+                            SEP() POST  [tptr tvoid]
+                            `(memory_block Tsh n0) retval)))
+                     (@PTree.Leaf global_spec)) (@None global_spec)
+                  (@PTree.Leaf global_spec))) (@None global_spec)
+            (@PTree.Node global_spec
+               (@PTree.Node global_spec
+                  (@PTree.Node global_spec (@PTree.Leaf global_spec)
+                     (@Some global_spec
+                        (Global_func
+                           (WITH _ : unit PRE  [(1%positive, tptr tschar),
+                            (2%positive, tint)](fun _ : environ => !!False)
+                            POST  [tint](fun _ : environ => !!False))))
+                     (@PTree.Node global_spec (@PTree.Leaf global_spec)
+                        (@Some global_spec
+                           (Global_func
+                              (WITH  q0 : val, contents0 : list val PRE 
+                               [(_Q, tptr t_struct_fifo)]
+                               PROP  ()
+                               LOCAL  (`(@eq val q0) (eval_id _Q))
+                               SEP  (`(fifo contents0 q0)) POST  [tint]
+                               (fun x0 : environ =>
+                                local
+                                  (`(@eq val
+                                       (if @isnil val contents0
+                                        then Vtrue
+                                        else Vfalse)) retval) x0 &&
+                                `(fifo contents0 q0) x0))))
+                        (@PTree.Leaf global_spec))) (@None global_spec)
+                  (@PTree.Leaf global_spec)) (@None global_spec)
+               (@PTree.Node global_spec
+                  (@PTree.Node global_spec (@PTree.Leaf global_spec)
+                     (@Some global_spec
+                        (Global_func
+                           (WITH _ : unit PRE  [(1%positive, tptr tvoid),
+                            (2%positive, tint)]
+                            PROP  ()
+                            LOCAL ()
+                            SEP 
+                            (`(memory_block Tsh)
+                               (`force_int (eval_id 2%positive))
+                               (eval_id 1%positive)) POST  [tvoid]
+                            (fun _ : environ => @emp mpred Nveric Sveric))))
+                     (@PTree.Node global_spec (@PTree.Leaf global_spec)
+                        (@Some global_spec
+                           (Global_func
+                              (WITH  p0 : val * list val, p1 : val PRE 
+                               [(_Q, tptr t_struct_fifo)]
+                               (let (q0, contents0) := p0 in
+                                PROP  ()
+                                LOCAL  (`(@eq val q0) (eval_id _Q))
+                                SEP  (`(fifo (p1 :: contents0) q0))) POST 
+                               [tptr t_struct_elem]
+                               (let (q0, contents0) := p0 in
+                                fun rho : environ =>
+                                local (`(@eq val p1) retval) rho &&
+                                `(fifo contents0 q0) rho * `link_ retval rho))))
+                        (@PTree.Leaf global_spec)))
+                  (@Some global_spec
+                     (Global_func
+                        (WITH _ : unit PRE  [(1%positive, tdouble)]
+                         (fun _ : environ => !!False) POST  [tdouble]
+                         (fun _ : environ => !!False))))
+                  (@PTree.Node global_spec (@PTree.Leaf global_spec)
+                     (@None global_spec)
+                     (@PTree.Node global_spec (@PTree.Leaf global_spec)
+                        (@Some global_spec
+                           (Global_func
+                              (WITH u : unit PRE  []main_pre prog u POST 
+                               [tint]main_post prog u)))
+                        (@PTree.Leaf global_spec)))))) in
+      PROP  ()
+      LOCAL  (tc_environ Delta; `(@eq val q) (eval_id _Q);
+      `(@eq val p) (eval_id _p))
+      SEP 
+      (@numbd (LiftEnviron mpred) 0
+         `(field_mapsto Tsh t_struct_fifo _head q hd);
+      @numbd (LiftEnviron mpred) 1
+        `(field_mapsto Tsh t_struct_fifo _tail q tl);
+      @numbd (LiftEnviron mpred) 2
+        `(if @isnil val contents
+          then !!(hd = nullval) && @emp mpred Nveric Sveric
+          else
+           EX  prefix : list val,
+           !!(contents = prefix ++ tl :: @nil val) &&
+           (@links t_struct_elem _next QS Tsh prefix hd tl * link tl nullval));
+      `(@numbd (lift_T (Tarrow val (LiftEnviron mpred))) 3
+          (field_mapsto_ Tsh t_struct_elem _next)) (eval_id _p))
+      |-- `(@numbd (val -> mpred) n
+              (field_mapsto_ sh
+                 (typeof
+                    (Ederef (Etempvar _p (tptr t_struct_elem)) t_struct_elem))
+                 _next))
+            (eval_lvalue
+               (Ederef (Etempvar _p (tptr t_struct_elem)) t_struct_elem)) *
+          @TT (LiftEnviron mpred) (@LiftNatDed' mpred Nveric)))
+. Proof. intros Q p h t; ungather_entail.
+unfold sh,n; entailer; cancel.
+Qed.
+
+Lemma goal_8 :
+name _Q ->
+name _p ->
+name _h ->
+name _t ->
+forall (q : val) (contents : list val) (p hd tl : val),
+let Delta :=
+  @abbreviate tycontext
+    (initialized _h
+       (@PTree.Node (type * bool)
+          (@PTree.Node (type * bool) (@PTree.Leaf (type * bool))
+             (@None (type * bool))
+             (@PTree.Node (type * bool) (@PTree.Leaf (type * bool))
+                (@None (type * bool))
+                (@PTree.Node (type * bool)
+                   (@PTree.Node (type * bool) (@PTree.Leaf (type * bool))
+                      (@Some (type * bool) (tptr t_struct_elem, false))
+                      (@PTree.Leaf (type * bool))) (@None (type * bool))
+                   (@PTree.Leaf (type * bool))))) (@None (type * bool))
+          (@PTree.Node (type * bool)
+             (@PTree.Node (type * bool) (@PTree.Leaf (type * bool))
+                (@None (type * bool))
+                (@PTree.Node (type * bool)
+                   (@PTree.Node (type * bool) (@PTree.Leaf (type * bool))
+                      (@Some (type * bool) (tptr t_struct_elem, true))
+                      (@PTree.Leaf (type * bool))) (@None (type * bool))
+                   (@PTree.Leaf (type * bool)))) (@None (type * bool))
+             (@PTree.Node (type * bool)
+                (@PTree.Node (type * bool)
+                   (@PTree.Node (type * bool) (@PTree.Leaf (type * bool))
+                      (@Some (type * bool) (tptr t_struct_fifo, true))
+                      (@PTree.Leaf (type * bool))) (@None (type * bool))
+                   (@PTree.Leaf (type * bool))) (@None (type * bool))
+                (@PTree.Node (type * bool)
+                   (@PTree.Node (type * bool) (@PTree.Leaf (type * bool))
+                      (@Some (type * bool) (tptr t_struct_elem, false))
+                      (@PTree.Leaf (type * bool))) (@None (type * bool))
+                   (@PTree.Leaf (type * bool))))), PTree.empty type, tvoid,
+       @PTree.Node global_spec
+         (@PTree.Node global_spec
+            (@PTree.Node global_spec
+               (@PTree.Node global_spec (@PTree.Leaf global_spec)
+                  (@Some global_spec
+                     (Global_func
+                        (WITH _ : unit PRE  [(1%positive, tptr tvoid),
+                         (2%positive, tptr tvoid), (3%positive, tuint),
+                         (4%positive, tuint)](fun _ : environ => !!False)
+                         POST  [tvoid](fun _ : environ => !!False))))
+                  (@PTree.Node global_spec (@PTree.Leaf global_spec)
+                     (@Some global_spec
+                        (Global_func
+                           (WITH  p0 : val * list val, p1 : val PRE 
+                            [(_Q, tptr t_struct_fifo),
+                            (_p, tptr t_struct_elem)]
+                            (let (q0, contents0) := p0 in
+                             PROP  ()
+                             LOCAL  (`(@eq val q0) (eval_id _Q);
+                             `(@eq val p1) (eval_id _p))
+                             SEP  (`(fifo contents0 q0); `(link_ p1))) POST 
+                            [tvoid]
+                            (let (q0, contents0) := p0 in
+                             `(fifo (contents0 ++ p1 :: @nil val) q0)))))
+                     (@PTree.Leaf global_spec))) (@None global_spec)
+               (@PTree.Node global_spec
+                  (@PTree.Node global_spec (@PTree.Leaf global_spec)
+                     (@Some global_spec
+                        (Global_func
+                           (WITH _ : unit PRE  []
+                            (fun _ : environ => @emp mpred Nveric Sveric)
+                            POST  [tptr t_struct_fifo]
+                            `(fifo (@nil val)) retval)))
+                     (@PTree.Leaf global_spec)) (@None global_spec)
+                  (@PTree.Node global_spec (@PTree.Leaf global_spec)
+                     (@Some global_spec
+                        (Global_func
+                           (WITH  a : int, b : int PRE  [(_a, tint),
+                            (_b, tint)]
+                            PROP  ()
+                            LOCAL  (`(@eq val (Vint a)) (eval_id _a);
+                            `(@eq val (Vint b)) (eval_id _b))  SEP() POST 
+                            [tptr t_struct_elem]`(elemrep (a, b)) retval)))
+                     (@PTree.Leaf global_spec)))) (@None global_spec)
+            (@PTree.Node global_spec
+               (@PTree.Node global_spec (@PTree.Leaf global_spec)
+                  (@Some global_spec
+                     (Global_func
+                        (WITH n : int PRE  [(1%positive, tint)]
+                         PROP  (4 <= Int.signed n)
+                         LOCAL  (`(@eq val (Vint n)) (eval_id 1%positive))
+                         SEP() POST  [tptr tvoid]`(memory_block Tsh n) retval)))
+                  (@PTree.Leaf global_spec)) (@None global_spec)
+               (@PTree.Leaf global_spec))) (@None global_spec)
+         (@PTree.Node global_spec
+            (@PTree.Node global_spec
+               (@PTree.Node global_spec (@PTree.Leaf global_spec)
+                  (@Some global_spec
+                     (Global_func
+                        (WITH _ : unit PRE  [(1%positive, tptr tschar),
+                         (2%positive, tint)](fun _ : environ => !!False)
+                         POST  [tint](fun _ : environ => !!False))))
+                  (@PTree.Node global_spec (@PTree.Leaf global_spec)
+                     (@Some global_spec
+                        (Global_func
+                           (WITH  q0 : val, contents0 : list val PRE 
+                            [(_Q, tptr t_struct_fifo)]
+                            PROP  ()
+                            LOCAL  (`(@eq val q0) (eval_id _Q))
+                            SEP  (`(fifo contents0 q0)) POST  [tint]
+                            (fun x0 : environ =>
+                             local
+                               (`(@eq val
+                                    (if @isnil val contents0
+                                     then Vtrue
+                                     else Vfalse)) retval) x0 &&
+                             `(fifo contents0 q0) x0))))
+                     (@PTree.Leaf global_spec))) (@None global_spec)
+               (@PTree.Leaf global_spec)) (@None global_spec)
+            (@PTree.Node global_spec
+               (@PTree.Node global_spec (@PTree.Leaf global_spec)
+                  (@Some global_spec
+                     (Global_func
+                        (WITH _ : unit PRE  [(1%positive, tptr tvoid),
+                         (2%positive, tint)]
+                         PROP  ()
+                         LOCAL ()
+                         SEP 
+                         (`(memory_block Tsh)
+                            (`force_int (eval_id 2%positive))
+                            (eval_id 1%positive)) POST  [tvoid]
+                         (fun _ : environ => @emp mpred Nveric Sveric))))
+                  (@PTree.Node global_spec (@PTree.Leaf global_spec)
+                     (@Some global_spec
+                        (Global_func
+                           (WITH  p0 : val * list val, p1 : val PRE 
+                            [(_Q, tptr t_struct_fifo)]
+                            (let (q0, contents0) := p0 in
+                             PROP  ()
+                             LOCAL  (`(@eq val q0) (eval_id _Q))
+                             SEP  (`(fifo (p1 :: contents0) q0))) POST 
+                            [tptr t_struct_elem]
+                            (let (q0, contents0) := p0 in
+                             fun rho : environ =>
+                             local (`(@eq val p1) retval) rho &&
+                             `(fifo contents0 q0) rho * `link_ retval rho))))
+                     (@PTree.Leaf global_spec)))
+               (@Some global_spec
+                  (Global_func
+                     (WITH _ : unit PRE  [(1%positive, tdouble)]
+                      (fun _ : environ => !!False) POST  [tdouble]
+                      (fun _ : environ => !!False))))
+               (@PTree.Node global_spec (@PTree.Leaf global_spec)
+                  (@None global_spec)
+                  (@PTree.Node global_spec (@PTree.Leaf global_spec)
+                     (@Some global_spec
+                        (Global_func
+                           (WITH u : unit PRE  []main_pre prog u POST  [tint]
+                            main_post prog u))) (@PTree.Leaf global_spec))))))) in
+PROP  ()
+LOCAL  (tc_environ Delta; `(@eq val hd) (eval_id _h);
+`(@eq val q) (eval_id _Q); `(@eq val p) (eval_id _p))
+SEP  (`(field_mapsto Tsh t_struct_fifo _head q hd);
+`(field_mapsto Tsh t_struct_fifo _tail q tl);
+`(if @isnil val contents
+  then !!(hd = nullval) && @emp mpred Nveric Sveric
+  else
+   EX  prefix : list val,
+   !!(contents = prefix ++ tl :: @nil val) &&
+   (@links t_struct_elem _next QS Tsh prefix hd tl * link tl nullval));
+`(field_mapsto Tsh
+    (Tstruct _struct_elem
+       (Fcons _a tint
+          (Fcons _b tint (Fcons _next (Tcomp_ptr _struct_elem noattr) Fnil)))
+       noattr) _next) (`force_ptr (eval_id _p)) `(Vint (Int.repr 0)))
+|-- PROP  ()
+    LOCAL 
+    (tc_expr Delta
+       (Ebinop Oeq (Etempvar _h (tptr t_struct_elem))
+          (Ecast (Econst_int (Int.repr 0) tint) (tptr tvoid)) tint);
+    `(@eq val hd) (eval_id _h); `(@eq val q) (eval_id _Q);
+    `(@eq val p) (eval_id _p))
+    SEP  (`(field_mapsto Tsh t_struct_fifo _head q hd);
+    `(field_mapsto Tsh t_struct_fifo _tail q tl);
+    `(if @isnil val contents
+      then !!(hd = nullval) && @emp mpred Nveric Sveric
+      else
+       EX  prefix : list val,
+       !!(contents = prefix ++ tl :: @nil val) &&
+       (@links t_struct_elem _next QS Tsh prefix hd tl * link tl nullval));
+    `(field_mapsto Tsh
+        (Tstruct _struct_elem
+           (Fcons _a tint
+              (Fcons _b tint
+                 (Fcons _next (Tcomp_ptr _struct_elem noattr) Fnil))) noattr)
+        _next) (`force_ptr (eval_id _p)) `(Vint (Int.repr 0)))
+. Proof.  intros Q p h t; ungather_entail.
+entailer!.
+Qed.
+
+Lemma goal_9 :
+name _Q ->
+name _p ->
+name _h ->
+name _t ->
+EVAR
+  (forall n : nat,
+   EVAR
+     (forall (sh : share) (q : val) (contents : list val) (p hd tl : val),
+      let Delta :=
+        @abbreviate tycontext
+          (initialized _h
+             (@PTree.Node (type * bool)
+                (@PTree.Node (type * bool) (@PTree.Leaf (type * bool))
+                   (@None (type * bool))
+                   (@PTree.Node (type * bool) (@PTree.Leaf (type * bool))
+                      (@None (type * bool))
+                      (@PTree.Node (type * bool)
+                         (@PTree.Node (type * bool)
+                            (@PTree.Leaf (type * bool))
+                            (@Some (type * bool) (tptr t_struct_elem, false))
+                            (@PTree.Leaf (type * bool)))
+                         (@None (type * bool)) (@PTree.Leaf (type * bool)))))
+                (@None (type * bool))
+                (@PTree.Node (type * bool)
+                   (@PTree.Node (type * bool) (@PTree.Leaf (type * bool))
+                      (@None (type * bool))
+                      (@PTree.Node (type * bool)
+                         (@PTree.Node (type * bool)
+                            (@PTree.Leaf (type * bool))
+                            (@Some (type * bool) (tptr t_struct_elem, true))
+                            (@PTree.Leaf (type * bool)))
+                         (@None (type * bool)) (@PTree.Leaf (type * bool))))
+                   (@None (type * bool))
+                   (@PTree.Node (type * bool)
+                      (@PTree.Node (type * bool)
+                         (@PTree.Node (type * bool)
+                            (@PTree.Leaf (type * bool))
+                            (@Some (type * bool) (tptr t_struct_fifo, true))
+                            (@PTree.Leaf (type * bool)))
+                         (@None (type * bool)) (@PTree.Leaf (type * bool)))
+                      (@None (type * bool))
+                      (@PTree.Node (type * bool)
+                         (@PTree.Node (type * bool)
+                            (@PTree.Leaf (type * bool))
+                            (@Some (type * bool) (tptr t_struct_elem, false))
+                            (@PTree.Leaf (type * bool)))
+                         (@None (type * bool)) (@PTree.Leaf (type * bool))))),
+             PTree.empty type, tvoid,
+             @PTree.Node global_spec
+               (@PTree.Node global_spec
+                  (@PTree.Node global_spec
+                     (@PTree.Node global_spec (@PTree.Leaf global_spec)
+                        (@Some global_spec
+                           (Global_func
+                              (WITH _ : unit PRE  [(1%positive, tptr tvoid),
+                               (2%positive, tptr tvoid), (3%positive, tuint),
+                               (4%positive, tuint)]
+                               (fun _ : environ => !!False) POST  [tvoid]
+                               (fun _ : environ => !!False))))
+                        (@PTree.Node global_spec (@PTree.Leaf global_spec)
+                           (@Some global_spec
+                              (Global_func
+                                 (WITH  p0 : val * list val, p1 : val PRE 
+                                  [(_Q, tptr t_struct_fifo),
+                                  (_p, tptr t_struct_elem)]
+                                  (let (q0, contents0) := p0 in
+                                   PROP  ()
+                                   LOCAL  (`(@eq val q0) (eval_id _Q);
+                                   `(@eq val p1) (eval_id _p))
+                                   SEP  (`(fifo contents0 q0); `(link_ p1)))
+                                  POST  [tvoid]
+                                  (let (q0, contents0) := p0 in
+                                   `(fifo (contents0 ++ p1 :: @nil val) q0)))))
+                           (@PTree.Leaf global_spec))) (@None global_spec)
+                     (@PTree.Node global_spec
+                        (@PTree.Node global_spec (@PTree.Leaf global_spec)
+                           (@Some global_spec
+                              (Global_func
+                                 (WITH _ : unit PRE  []
+                                  (fun _ : environ =>
+                                   @emp mpred Nveric Sveric) POST 
+                                  [tptr t_struct_fifo]
+                                  `(fifo (@nil val)) retval)))
+                           (@PTree.Leaf global_spec)) (@None global_spec)
+                        (@PTree.Node global_spec (@PTree.Leaf global_spec)
+                           (@Some global_spec
+                              (Global_func
+                                 (WITH  a : int, b : int PRE  [(_a, tint),
+                                  (_b, tint)]
+                                  PROP  ()
+                                  LOCAL  (`(@eq val (Vint a)) (eval_id _a);
+                                  `(@eq val (Vint b)) (eval_id _b))  
+                                  SEP() POST  [tptr t_struct_elem]
+                                  `(elemrep (a, b)) retval)))
+                           (@PTree.Leaf global_spec)))) (@None global_spec)
+                  (@PTree.Node global_spec
+                     (@PTree.Node global_spec (@PTree.Leaf global_spec)
+                        (@Some global_spec
+                           (Global_func
+                              (WITH n0 : int PRE  [(1%positive, tint)]
+                               PROP  (4 <= Int.signed n0)
+                               LOCAL 
+                               (`(@eq val (Vint n0)) (eval_id 1%positive))
+                               SEP() POST  [tptr tvoid]
+                               `(memory_block Tsh n0) retval)))
+                        (@PTree.Leaf global_spec)) (@None global_spec)
+                     (@PTree.Leaf global_spec))) (@None global_spec)
+               (@PTree.Node global_spec
+                  (@PTree.Node global_spec
+                     (@PTree.Node global_spec (@PTree.Leaf global_spec)
+                        (@Some global_spec
+                           (Global_func
+                              (WITH _ : unit PRE  [(1%positive, tptr tschar),
+                               (2%positive, tint)]
+                               (fun _ : environ => !!False) POST  [tint]
+                               (fun _ : environ => !!False))))
+                        (@PTree.Node global_spec (@PTree.Leaf global_spec)
+                           (@Some global_spec
+                              (Global_func
+                                 (WITH  q0 : val, contents0 : list val PRE 
+                                  [(_Q, tptr t_struct_fifo)]
+                                  PROP  ()
+                                  LOCAL  (`(@eq val q0) (eval_id _Q))
+                                  SEP  (`(fifo contents0 q0)) POST  [tint]
+                                  (fun x0 : environ =>
+                                   local
+                                     (`(@eq val
+                                          (if @isnil val contents0
+                                           then Vtrue
+                                           else Vfalse)) retval) x0 &&
+                                   `(fifo contents0 q0) x0))))
+                           (@PTree.Leaf global_spec))) (@None global_spec)
+                     (@PTree.Leaf global_spec)) (@None global_spec)
+                  (@PTree.Node global_spec
+                     (@PTree.Node global_spec (@PTree.Leaf global_spec)
+                        (@Some global_spec
+                           (Global_func
+                              (WITH _ : unit PRE  [(1%positive, tptr tvoid),
+                               (2%positive, tint)]
+                               PROP  ()
+                               LOCAL ()
+                               SEP 
+                               (`(memory_block Tsh)
+                                  (`force_int (eval_id 2%positive))
+                                  (eval_id 1%positive)) POST  [tvoid]
+                               (fun _ : environ => @emp mpred Nveric Sveric))))
+                        (@PTree.Node global_spec (@PTree.Leaf global_spec)
+                           (@Some global_spec
+                              (Global_func
+                                 (WITH  p0 : val * list val, p1 : val PRE 
+                                  [(_Q, tptr t_struct_fifo)]
+                                  (let (q0, contents0) := p0 in
+                                   PROP  ()
+                                   LOCAL  (`(@eq val q0) (eval_id _Q))
+                                   SEP  (`(fifo (p1 :: contents0) q0))) POST 
+                                  [tptr t_struct_elem]
+                                  (let (q0, contents0) := p0 in
+                                   fun rho : environ =>
+                                   local (`(@eq val p1) retval) rho &&
+                                   `(fifo contents0 q0) rho *
+                                   `link_ retval rho))))
+                           (@PTree.Leaf global_spec)))
+                     (@Some global_spec
+                        (Global_func
+                           (WITH _ : unit PRE  [(1%positive, tdouble)]
+                            (fun _ : environ => !!False) POST  [tdouble]
+                            (fun _ : environ => !!False))))
+                     (@PTree.Node global_spec (@PTree.Leaf global_spec)
+                        (@None global_spec)
+                        (@PTree.Node global_spec (@PTree.Leaf global_spec)
+                           (@Some global_spec
+                              (Global_func
+                                 (WITH u : unit PRE  []main_pre prog u POST 
+                                  [tint]main_post prog u)))
+                           (@PTree.Leaf global_spec))))))) in
+      PROP  ()
+      LOCAL  (tc_environ Delta;
+      `(typed_true
+          (typeof
+             (Ebinop Oeq (Etempvar _h (tptr t_struct_elem))
+                (Ecast (Econst_int (Int.repr 0) tint) (tptr tvoid)) tint)))
+        (eval_expr
+           (Ebinop Oeq (Etempvar _h (tptr t_struct_elem))
+              (Ecast (Econst_int (Int.repr 0) tint) (tptr tvoid)) tint));
+      `(@eq val hd) (eval_id _h); `(@eq val q) (eval_id _Q);
+      `(@eq val p) (eval_id _p))
+      SEP 
+      (@numbd (LiftEnviron mpred) 0
+         `(field_mapsto Tsh t_struct_fifo _head q hd);
+      @numbd (LiftEnviron mpred) 1
+        `(field_mapsto Tsh t_struct_fifo _tail q tl);
+      @numbd (LiftEnviron mpred) 2
+        `(if @isnil val contents
+          then !!(hd = nullval) && @emp mpred Nveric Sveric
+          else
+           EX  prefix : list val,
+           !!(contents = prefix ++ tl :: @nil val) &&
+           (@links t_struct_elem _next QS Tsh prefix hd tl * link tl nullval));
+      `(@numbd (lift_T (Tarrow val (Tarrow val (LiftEnviron mpred)))) 3
+          (field_mapsto Tsh
+             (Tstruct _struct_elem
+                (Fcons _a tint
+                   (Fcons _b tint
+                      (Fcons _next (Tcomp_ptr _struct_elem noattr) Fnil)))
+                noattr) _next)) (`force_ptr (eval_id _p))
+        `(Vint (Int.repr 0)))
+      |-- `(@numbd (val -> mpred) n
+              (field_mapsto_ sh
+                 (typeof
+                    (Ederef (Etempvar _Q (tptr t_struct_fifo)) t_struct_fifo))
+                 _head))
+            (eval_lvalue
+               (Ederef (Etempvar _Q (tptr t_struct_fifo)) t_struct_fifo)) *
+          @TT (LiftEnviron mpred) (@LiftNatDed' mpred Nveric)))
+. Proof. intros Q p h t; ungather_entail.
+unfold n,sh. entailer. cancel.
+Qed.
+
+Lemma goal_10 :
+name _Q ->
+name _p ->
+name _h ->
+name _t ->
+forall (q : val) (contents : list val) (p hd tl : val),
+let Delta :=
+  @abbreviate tycontext
+    (initialized _h
+       (@PTree.Node (type * bool)
+          (@PTree.Node (type * bool) (@PTree.Leaf (type * bool))
+             (@None (type * bool))
+             (@PTree.Node (type * bool) (@PTree.Leaf (type * bool))
+                (@None (type * bool))
+                (@PTree.Node (type * bool)
+                   (@PTree.Node (type * bool) (@PTree.Leaf (type * bool))
+                      (@Some (type * bool) (tptr t_struct_elem, false))
+                      (@PTree.Leaf (type * bool))) (@None (type * bool))
+                   (@PTree.Leaf (type * bool))))) (@None (type * bool))
+          (@PTree.Node (type * bool)
+             (@PTree.Node (type * bool) (@PTree.Leaf (type * bool))
+                (@None (type * bool))
+                (@PTree.Node (type * bool)
+                   (@PTree.Node (type * bool) (@PTree.Leaf (type * bool))
+                      (@Some (type * bool) (tptr t_struct_elem, true))
+                      (@PTree.Leaf (type * bool))) (@None (type * bool))
+                   (@PTree.Leaf (type * bool)))) (@None (type * bool))
+             (@PTree.Node (type * bool)
+                (@PTree.Node (type * bool)
+                   (@PTree.Node (type * bool) (@PTree.Leaf (type * bool))
+                      (@Some (type * bool) (tptr t_struct_fifo, true))
+                      (@PTree.Leaf (type * bool))) (@None (type * bool))
+                   (@PTree.Leaf (type * bool))) (@None (type * bool))
+                (@PTree.Node (type * bool)
+                   (@PTree.Node (type * bool) (@PTree.Leaf (type * bool))
+                      (@Some (type * bool) (tptr t_struct_elem, false))
+                      (@PTree.Leaf (type * bool))) (@None (type * bool))
+                   (@PTree.Leaf (type * bool))))), PTree.empty type, tvoid,
+       @PTree.Node global_spec
+         (@PTree.Node global_spec
+            (@PTree.Node global_spec
+               (@PTree.Node global_spec (@PTree.Leaf global_spec)
+                  (@Some global_spec
+                     (Global_func
+                        (WITH _ : unit PRE  [(1%positive, tptr tvoid),
+                         (2%positive, tptr tvoid), (3%positive, tuint),
+                         (4%positive, tuint)](fun _ : environ => !!False)
+                         POST  [tvoid](fun _ : environ => !!False))))
+                  (@PTree.Node global_spec (@PTree.Leaf global_spec)
+                     (@Some global_spec
+                        (Global_func
+                           (WITH  p0 : val * list val, p1 : val PRE 
+                            [(_Q, tptr t_struct_fifo),
+                            (_p, tptr t_struct_elem)]
+                            (let (q0, contents0) := p0 in
+                             PROP  ()
+                             LOCAL  (`(@eq val q0) (eval_id _Q);
+                             `(@eq val p1) (eval_id _p))
+                             SEP  (`(fifo contents0 q0); `(link_ p1))) POST 
+                            [tvoid]
+                            (let (q0, contents0) := p0 in
+                             `(fifo (contents0 ++ p1 :: @nil val) q0)))))
+                     (@PTree.Leaf global_spec))) (@None global_spec)
+               (@PTree.Node global_spec
+                  (@PTree.Node global_spec (@PTree.Leaf global_spec)
+                     (@Some global_spec
+                        (Global_func
+                           (WITH _ : unit PRE  []
+                            (fun _ : environ => @emp mpred Nveric Sveric)
+                            POST  [tptr t_struct_fifo]
+                            `(fifo (@nil val)) retval)))
+                     (@PTree.Leaf global_spec)) (@None global_spec)
+                  (@PTree.Node global_spec (@PTree.Leaf global_spec)
+                     (@Some global_spec
+                        (Global_func
+                           (WITH  a : int, b : int PRE  [(_a, tint),
+                            (_b, tint)]
+                            PROP  ()
+                            LOCAL  (`(@eq val (Vint a)) (eval_id _a);
+                            `(@eq val (Vint b)) (eval_id _b))  SEP() POST 
+                            [tptr t_struct_elem]`(elemrep (a, b)) retval)))
+                     (@PTree.Leaf global_spec)))) (@None global_spec)
+            (@PTree.Node global_spec
+               (@PTree.Node global_spec (@PTree.Leaf global_spec)
+                  (@Some global_spec
+                     (Global_func
+                        (WITH n : int PRE  [(1%positive, tint)]
+                         PROP  (4 <= Int.signed n)
+                         LOCAL  (`(@eq val (Vint n)) (eval_id 1%positive))
+                         SEP() POST  [tptr tvoid]`(memory_block Tsh n) retval)))
+                  (@PTree.Leaf global_spec)) (@None global_spec)
+               (@PTree.Leaf global_spec))) (@None global_spec)
+         (@PTree.Node global_spec
+            (@PTree.Node global_spec
+               (@PTree.Node global_spec (@PTree.Leaf global_spec)
+                  (@Some global_spec
+                     (Global_func
+                        (WITH _ : unit PRE  [(1%positive, tptr tschar),
+                         (2%positive, tint)](fun _ : environ => !!False)
+                         POST  [tint](fun _ : environ => !!False))))
+                  (@PTree.Node global_spec (@PTree.Leaf global_spec)
+                     (@Some global_spec
+                        (Global_func
+                           (WITH  q0 : val, contents0 : list val PRE 
+                            [(_Q, tptr t_struct_fifo)]
+                            PROP  ()
+                            LOCAL  (`(@eq val q0) (eval_id _Q))
+                            SEP  (`(fifo contents0 q0)) POST  [tint]
+                            (fun x0 : environ =>
+                             local
+                               (`(@eq val
+                                    (if @isnil val contents0
+                                     then Vtrue
+                                     else Vfalse)) retval) x0 &&
+                             `(fifo contents0 q0) x0))))
+                     (@PTree.Leaf global_spec))) (@None global_spec)
+               (@PTree.Leaf global_spec)) (@None global_spec)
+            (@PTree.Node global_spec
+               (@PTree.Node global_spec (@PTree.Leaf global_spec)
+                  (@Some global_spec
+                     (Global_func
+                        (WITH _ : unit PRE  [(1%positive, tptr tvoid),
+                         (2%positive, tint)]
+                         PROP  ()
+                         LOCAL ()
+                         SEP 
+                         (`(memory_block Tsh)
+                            (`force_int (eval_id 2%positive))
+                            (eval_id 1%positive)) POST  [tvoid]
+                         (fun _ : environ => @emp mpred Nveric Sveric))))
+                  (@PTree.Node global_spec (@PTree.Leaf global_spec)
+                     (@Some global_spec
+                        (Global_func
+                           (WITH  p0 : val * list val, p1 : val PRE 
+                            [(_Q, tptr t_struct_fifo)]
+                            (let (q0, contents0) := p0 in
+                             PROP  ()
+                             LOCAL  (`(@eq val q0) (eval_id _Q))
+                             SEP  (`(fifo (p1 :: contents0) q0))) POST 
+                            [tptr t_struct_elem]
+                            (let (q0, contents0) := p0 in
+                             fun rho : environ =>
+                             local (`(@eq val p1) retval) rho &&
+                             `(fifo contents0 q0) rho * `link_ retval rho))))
+                     (@PTree.Leaf global_spec)))
+               (@Some global_spec
+                  (Global_func
+                     (WITH _ : unit PRE  [(1%positive, tdouble)]
+                      (fun _ : environ => !!False) POST  [tdouble]
+                      (fun _ : environ => !!False))))
+               (@PTree.Node global_spec (@PTree.Leaf global_spec)
+                  (@None global_spec)
+                  (@PTree.Node global_spec (@PTree.Leaf global_spec)
+                     (@Some global_spec
+                        (Global_func
+                           (WITH u : unit PRE  []main_pre prog u POST  [tint]
+                            main_post prog u))) (@PTree.Leaf global_spec))))))) in
+PROP  ()
+LOCAL  (tc_environ Delta;
+`(typed_true
+    (typeof
+       (Ebinop Oeq (Etempvar _h (tptr t_struct_elem))
+          (Ecast (Econst_int (Int.repr 0) tint) (tptr tvoid)) tint)))
+  (eval_expr
+     (Ebinop Oeq (Etempvar _h (tptr t_struct_elem))
+        (Ecast (Econst_int (Int.repr 0) tint) (tptr tvoid)) tint));
+`(@eq val hd) (eval_id _h); `(@eq val q) (eval_id _Q);
+`(@eq val p) (eval_id _p))
+SEP 
+(`(field_mapsto Tsh
+     (Tstruct _struct_fifo
+        (Fcons _head
+           (tptr
+              (Tstruct _struct_elem
+                 (Fcons _a tint
+                    (Fcons _b tint
+                       (Fcons _next (Tcomp_ptr _struct_elem noattr) Fnil)))
+                 noattr))
+           (Fcons _tail
+              (tptr
+                 (Tstruct _struct_elem
+                    (Fcons _a tint
+                       (Fcons _b tint
+                          (Fcons _next (Tcomp_ptr _struct_elem noattr) Fnil)))
+                    noattr)) Fnil)) noattr) _head)
+   (eval_lvalue (Ederef (Etempvar _Q (tptr t_struct_fifo)) t_struct_fifo))
+   (`(eval_cast (typeof (Etempvar _p (tptr t_struct_elem)))
+        (tptr t_struct_elem)) (eval_expr (Etempvar _p (tptr t_struct_elem))));
+`(field_mapsto Tsh
+    (Tstruct _struct_fifo
+       (Fcons _head
+          (tptr
+             (Tstruct _struct_elem
+                (Fcons _a tint
+                   (Fcons _b tint
+                      (Fcons _next (Tcomp_ptr _struct_elem noattr) Fnil)))
+                noattr))
+          (Fcons _tail
+             (tptr
+                (Tstruct _struct_elem
+                   (Fcons _a tint
+                      (Fcons _b tint
+                         (Fcons _next (Tcomp_ptr _struct_elem noattr) Fnil)))
+                   noattr)) Fnil)) noattr) _tail)
+  (eval_lvalue (Ederef (Etempvar _Q (tptr t_struct_fifo)) t_struct_fifo))
+  (`(eval_cast (typeof (Etempvar _p (tptr t_struct_elem)))
+       (tptr t_struct_elem)) (eval_expr (Etempvar _p (tptr t_struct_elem))));
+`(if @isnil val contents
+  then !!(hd = nullval) && @emp mpred Nveric Sveric
+  else
+   EX  prefix : list val,
+   !!(contents = prefix ++ tl :: @nil val) &&
+   (@links t_struct_elem _next QS Tsh prefix hd tl * link tl nullval));
+`(field_mapsto Tsh
+    (Tstruct _struct_elem
+       (Fcons _a tint
+          (Fcons _b tint (Fcons _next (Tcomp_ptr _struct_elem noattr) Fnil)))
+       noattr) _next) (`force_ptr (eval_id _p)) `(Vint (Int.repr 0)))
+|-- overridePost
+      (PROP  ()  LOCAL ()  SEP  (`(fifo (contents ++ p :: @nil val) q)))
+      (function_body_ret_assert tvoid `(fifo (contents ++ p :: @nil val) q))
+      EK_normal (@None val)
+. Proof. intros Q p' h t; ungather_entail.
+entailer.
+  destruct (@isnil val contents).
+  + subst. unfold fifo. apply exp_right with (p',p').  
+      simpl.
+      destruct (isnil (p' ::nil)); [ congruence | ].
+      normalize.
+      apply exp_right with nil.
+      simpl. rewrite links_nil_eq.
+      entailer!.
+  + unfold link.
+      normalize.
+      destruct prefix.
+      - rewrite links_nil_eq.
+         normalize.
+         apply ptr_eq_e in H4. subst tl.
+         entailer.
+         destruct h; inv H4; inv H0.
+      - rewrite links_cons_eq.
+         normalize.
+do 2 rewrite <- sepcon_assoc. (* this line shouldn't be necessary before saturate_local *)
+         entailer.
+         destruct v; inv H7; inv H0.
+Qed.
+
+Lemma goal_11 :
+name _Q ->
+name _p ->
+name _h ->
+name _t ->
+forall (q : val) (contents : list val) (p hd tl : val),
+contents = @nil val ->
+let Delta :=
+  @abbreviate tycontext
+    (initialized _t
+       (initialized _h
+          (@PTree.Node (type * bool)
+             (@PTree.Node (type * bool) (@PTree.Leaf (type * bool))
+                (@None (type * bool))
+                (@PTree.Node (type * bool) (@PTree.Leaf (type * bool))
+                   (@None (type * bool))
+                   (@PTree.Node (type * bool)
+                      (@PTree.Node (type * bool) (@PTree.Leaf (type * bool))
+                         (@Some (type * bool) (tptr t_struct_elem, false))
+                         (@PTree.Leaf (type * bool))) (@None (type * bool))
+                      (@PTree.Leaf (type * bool))))) (@None (type * bool))
+             (@PTree.Node (type * bool)
+                (@PTree.Node (type * bool) (@PTree.Leaf (type * bool))
+                   (@None (type * bool))
+                   (@PTree.Node (type * bool)
+                      (@PTree.Node (type * bool) (@PTree.Leaf (type * bool))
+                         (@Some (type * bool) (tptr t_struct_elem, true))
+                         (@PTree.Leaf (type * bool))) (@None (type * bool))
+                      (@PTree.Leaf (type * bool)))) (@None (type * bool))
+                (@PTree.Node (type * bool)
+                   (@PTree.Node (type * bool)
+                      (@PTree.Node (type * bool) (@PTree.Leaf (type * bool))
+                         (@Some (type * bool) (tptr t_struct_fifo, true))
+                         (@PTree.Leaf (type * bool))) (@None (type * bool))
+                      (@PTree.Leaf (type * bool))) (@None (type * bool))
+                   (@PTree.Node (type * bool)
+                      (@PTree.Node (type * bool) (@PTree.Leaf (type * bool))
+                         (@Some (type * bool) (tptr t_struct_elem, false))
+                         (@PTree.Leaf (type * bool))) (@None (type * bool))
+                      (@PTree.Leaf (type * bool))))), PTree.empty type,
+          tvoid,
+          @PTree.Node global_spec
+            (@PTree.Node global_spec
+               (@PTree.Node global_spec
+                  (@PTree.Node global_spec (@PTree.Leaf global_spec)
+                     (@Some global_spec
+                        (Global_func
+                           (WITH _ : unit PRE  [(1%positive, tptr tvoid),
+                            (2%positive, tptr tvoid), (3%positive, tuint),
+                            (4%positive, tuint)](fun _ : environ => !!False)
+                            POST  [tvoid](fun _ : environ => !!False))))
+                     (@PTree.Node global_spec (@PTree.Leaf global_spec)
+                        (@Some global_spec
+                           (Global_func
+                              (WITH  p0 : val * list val, p1 : val PRE 
+                               [(_Q, tptr t_struct_fifo),
+                               (_p, tptr t_struct_elem)]
+                               (let (q0, contents0) := p0 in
+                                PROP  ()
+                                LOCAL  (`(@eq val q0) (eval_id _Q);
+                                `(@eq val p1) (eval_id _p))
+                                SEP  (`(fifo contents0 q0); `(link_ p1)))
+                               POST  [tvoid]
+                               (let (q0, contents0) := p0 in
+                                `(fifo (contents0 ++ p1 :: @nil val) q0)))))
+                        (@PTree.Leaf global_spec))) (@None global_spec)
+                  (@PTree.Node global_spec
+                     (@PTree.Node global_spec (@PTree.Leaf global_spec)
+                        (@Some global_spec
+                           (Global_func
+                              (WITH _ : unit PRE  []
+                               (fun _ : environ => @emp mpred Nveric Sveric)
+                               POST  [tptr t_struct_fifo]
+                               `(fifo (@nil val)) retval)))
+                        (@PTree.Leaf global_spec)) (@None global_spec)
+                     (@PTree.Node global_spec (@PTree.Leaf global_spec)
+                        (@Some global_spec
+                           (Global_func
+                              (WITH  a : int, b : int PRE  [(_a, tint),
+                               (_b, tint)]
+                               PROP  ()
+                               LOCAL  (`(@eq val (Vint a)) (eval_id _a);
+                               `(@eq val (Vint b)) (eval_id _b))  SEP() POST 
+                               [tptr t_struct_elem]`(elemrep (a, b)) retval)))
+                        (@PTree.Leaf global_spec)))) (@None global_spec)
+               (@PTree.Node global_spec
+                  (@PTree.Node global_spec (@PTree.Leaf global_spec)
+                     (@Some global_spec
+                        (Global_func
+                           (WITH n : int PRE  [(1%positive, tint)]
+                            PROP  (4 <= Int.signed n)
+                            LOCAL  (`(@eq val (Vint n)) (eval_id 1%positive))
+                              SEP() POST  [tptr tvoid]
+                            `(memory_block Tsh n) retval)))
+                     (@PTree.Leaf global_spec)) (@None global_spec)
+                  (@PTree.Leaf global_spec))) (@None global_spec)
+            (@PTree.Node global_spec
+               (@PTree.Node global_spec
+                  (@PTree.Node global_spec (@PTree.Leaf global_spec)
+                     (@Some global_spec
+                        (Global_func
+                           (WITH _ : unit PRE  [(1%positive, tptr tschar),
+                            (2%positive, tint)](fun _ : environ => !!False)
+                            POST  [tint](fun _ : environ => !!False))))
+                     (@PTree.Node global_spec (@PTree.Leaf global_spec)
+                        (@Some global_spec
+                           (Global_func
+                              (WITH  q0 : val, contents0 : list val PRE 
+                               [(_Q, tptr t_struct_fifo)]
+                               PROP  ()
+                               LOCAL  (`(@eq val q0) (eval_id _Q))
+                               SEP  (`(fifo contents0 q0)) POST  [tint]
+                               (fun x0 : environ =>
+                                local
+                                  (`(@eq val
+                                       (if @isnil val contents0
+                                        then Vtrue
+                                        else Vfalse)) retval) x0 &&
+                                `(fifo contents0 q0) x0))))
+                        (@PTree.Leaf global_spec))) (@None global_spec)
+                  (@PTree.Leaf global_spec)) (@None global_spec)
+               (@PTree.Node global_spec
+                  (@PTree.Node global_spec (@PTree.Leaf global_spec)
+                     (@Some global_spec
+                        (Global_func
+                           (WITH _ : unit PRE  [(1%positive, tptr tvoid),
+                            (2%positive, tint)]
+                            PROP  ()
+                            LOCAL ()
+                            SEP 
+                            (`(memory_block Tsh)
+                               (`force_int (eval_id 2%positive))
+                               (eval_id 1%positive)) POST  [tvoid]
+                            (fun _ : environ => @emp mpred Nveric Sveric))))
+                     (@PTree.Node global_spec (@PTree.Leaf global_spec)
+                        (@Some global_spec
+                           (Global_func
+                              (WITH  p0 : val * list val, p1 : val PRE 
+                               [(_Q, tptr t_struct_fifo)]
+                               (let (q0, contents0) := p0 in
+                                PROP  ()
+                                LOCAL  (`(@eq val q0) (eval_id _Q))
+                                SEP  (`(fifo (p1 :: contents0) q0))) POST 
+                               [tptr t_struct_elem]
+                               (let (q0, contents0) := p0 in
+                                fun rho : environ =>
+                                local (`(@eq val p1) retval) rho &&
+                                `(fifo contents0 q0) rho * `link_ retval rho))))
+                        (@PTree.Leaf global_spec)))
+                  (@Some global_spec
+                     (Global_func
+                        (WITH _ : unit PRE  [(1%positive, tdouble)]
+                         (fun _ : environ => !!False) POST  [tdouble]
+                         (fun _ : environ => !!False))))
+                  (@PTree.Node global_spec (@PTree.Leaf global_spec)
+                     (@None global_spec)
+                     (@PTree.Node global_spec (@PTree.Leaf global_spec)
+                        (@Some global_spec
+                           (Global_func
+                              (WITH u : unit PRE  []main_pre prog u POST 
+                               [tint]main_post prog u)))
+                        (@PTree.Leaf global_spec)))))))) in
+PROP  ()
+LOCAL  (tc_environ Delta; `(@eq val tl) (eval_id _t);
+`(typed_false
+    (typeof
+       (Ebinop Oeq (Etempvar _h (tptr t_struct_elem))
+          (Ecast (Econst_int (Int.repr 0) tint) (tptr tvoid)) tint)))
+  (eval_expr
+     (Ebinop Oeq (Etempvar _h (tptr t_struct_elem))
+        (Ecast (Econst_int (Int.repr 0) tint) (tptr tvoid)) tint));
+`(@eq val hd) (eval_id _h); `(@eq val q) (eval_id _Q);
+`(@eq val p) (eval_id _p))
+SEP  (`(field_mapsto Tsh t_struct_fifo _head q hd);
+`(field_mapsto Tsh t_struct_fifo _tail q tl);
+`(!!(hd = nullval) && @emp mpred Nveric Sveric);
+`(field_mapsto Tsh
+    (Tstruct _struct_elem
+       (Fcons _a tint
+          (Fcons _b tint (Fcons _next (Tcomp_ptr _struct_elem noattr) Fnil)))
+       noattr) _next) (`force_ptr (eval_id _p)) `(Vint (Int.repr 0)))
+|-- @FF (environ -> mpred) (@LiftNatDed' mpred Nveric)
+. Proof. intros Q p' h t; ungather_entail.
+entailer. inv H2.
+Qed.
+
+Lemma goal_12 :
+name _Q ->
+name _p ->
+name _h ->
+name _t ->
+EVAR
+  (forall n0 : nat,
+   EVAR
+     (forall (sh : share) (q : val) (contents : list val) (p hd tl : val),
+      contents <> @nil val ->
+      forall prefix : list val,
+      contents = prefix ++ tl :: @nil val ->
+      let Delta :=
+        @abbreviate tycontext
+          (initialized _t
+             (initialized _h
+                (@PTree.Node (type * bool)
+                   (@PTree.Node (type * bool) (@PTree.Leaf (type * bool))
+                      (@None (type * bool))
+                      (@PTree.Node (type * bool) (@PTree.Leaf (type * bool))
+                         (@None (type * bool))
+                         (@PTree.Node (type * bool)
+                            (@PTree.Node (type * bool)
+                               (@PTree.Leaf (type * bool))
+                               (@Some (type * bool)
+                                  (tptr t_struct_elem, false))
+                               (@PTree.Leaf (type * bool)))
+                            (@None (type * bool)) (@PTree.Leaf (type * bool)))))
+                   (@None (type * bool))
+                   (@PTree.Node (type * bool)
+                      (@PTree.Node (type * bool) (@PTree.Leaf (type * bool))
+                         (@None (type * bool))
+                         (@PTree.Node (type * bool)
+                            (@PTree.Node (type * bool)
+                               (@PTree.Leaf (type * bool))
+                               (@Some (type * bool)
+                                  (tptr t_struct_elem, true))
+                               (@PTree.Leaf (type * bool)))
+                            (@None (type * bool)) (@PTree.Leaf (type * bool))))
+                      (@None (type * bool))
+                      (@PTree.Node (type * bool)
+                         (@PTree.Node (type * bool)
+                            (@PTree.Node (type * bool)
+                               (@PTree.Leaf (type * bool))
+                               (@Some (type * bool)
+                                  (tptr t_struct_fifo, true))
+                               (@PTree.Leaf (type * bool)))
+                            (@None (type * bool)) (@PTree.Leaf (type * bool)))
+                         (@None (type * bool))
+                         (@PTree.Node (type * bool)
+                            (@PTree.Node (type * bool)
+                               (@PTree.Leaf (type * bool))
+                               (@Some (type * bool)
+                                  (tptr t_struct_elem, false))
+                               (@PTree.Leaf (type * bool)))
+                            (@None (type * bool)) (@PTree.Leaf (type * bool))))),
+                PTree.empty type, tvoid,
+                @PTree.Node global_spec
+                  (@PTree.Node global_spec
+                     (@PTree.Node global_spec
+                        (@PTree.Node global_spec (@PTree.Leaf global_spec)
+                           (@Some global_spec
+                              (Global_func
+                                 (WITH _ : unit PRE 
+                                  [(1%positive, tptr tvoid),
+                                  (2%positive, tptr tvoid),
+                                  (3%positive, tuint), (4%positive, tuint)]
+                                  (fun _ : environ => !!False) POST  [tvoid]
+                                  (fun _ : environ => !!False))))
+                           (@PTree.Node global_spec (@PTree.Leaf global_spec)
+                              (@Some global_spec
+                                 (Global_func
+                                    (WITH  p0 : val * list val, p1 : val PRE 
+                                     [(_Q, tptr t_struct_fifo),
+                                     (_p, tptr t_struct_elem)]
+                                     (let (q0, contents0) := p0 in
+                                      PROP  ()
+                                      LOCAL  (`(@eq val q0) (eval_id _Q);
+                                      `(@eq val p1) (eval_id _p))
+                                      SEP  (`(fifo contents0 q0);
+                                      `(link_ p1))) POST  [tvoid]
+                                     (let (q0, contents0) := p0 in
+                                      `(fifo (contents0 ++ p1 :: @nil val) q0)))))
+                              (@PTree.Leaf global_spec))) (@None global_spec)
+                        (@PTree.Node global_spec
+                           (@PTree.Node global_spec (@PTree.Leaf global_spec)
+                              (@Some global_spec
+                                 (Global_func
+                                    (WITH _ : unit PRE  []
+                                     (fun _ : environ =>
+                                      @emp mpred Nveric Sveric) POST 
+                                     [tptr t_struct_fifo]
+                                     `(fifo (@nil val)) retval)))
+                              (@PTree.Leaf global_spec)) (@None global_spec)
+                           (@PTree.Node global_spec (@PTree.Leaf global_spec)
+                              (@Some global_spec
+                                 (Global_func
+                                    (WITH  a : int, b : int PRE  [(_a, tint),
+                                     (_b, tint)]
+                                     PROP  ()
+                                     LOCAL 
+                                     (`(@eq val (Vint a)) (eval_id _a);
+                                     `(@eq val (Vint b)) (eval_id _b))  
+                                     SEP() POST  [tptr t_struct_elem]
+                                     `(elemrep (a, b)) retval)))
+                              (@PTree.Leaf global_spec))))
+                     (@None global_spec)
+                     (@PTree.Node global_spec
+                        (@PTree.Node global_spec (@PTree.Leaf global_spec)
+                           (@Some global_spec
+                              (Global_func
+                                 (WITH n1 : int PRE  [(1%positive, tint)]
+                                  PROP  (4 <= Int.signed n1)
+                                  LOCAL 
+                                  (`(@eq val (Vint n1)) (eval_id 1%positive))
+                                    SEP() POST  [tptr tvoid]
+                                  `(memory_block Tsh n1) retval)))
+                           (@PTree.Leaf global_spec)) (@None global_spec)
+                        (@PTree.Leaf global_spec))) (@None global_spec)
+                  (@PTree.Node global_spec
+                     (@PTree.Node global_spec
+                        (@PTree.Node global_spec (@PTree.Leaf global_spec)
+                           (@Some global_spec
+                              (Global_func
+                                 (WITH _ : unit PRE 
+                                  [(1%positive, tptr tschar),
+                                  (2%positive, tint)]
+                                  (fun _ : environ => !!False) POST  [tint]
+                                  (fun _ : environ => !!False))))
+                           (@PTree.Node global_spec (@PTree.Leaf global_spec)
+                              (@Some global_spec
+                                 (Global_func
+                                    (WITH  q0 : val, contents0 : list val
+                                     PRE  [(_Q, tptr t_struct_fifo)]
+                                     PROP  ()
+                                     LOCAL  (`(@eq val q0) (eval_id _Q))
+                                     SEP  (`(fifo contents0 q0)) POST  [tint]
+                                     (fun x0 : environ =>
+                                      local
+                                        (`(@eq val
+                                             (if @isnil val contents0
+                                              then Vtrue
+                                              else Vfalse)) retval) x0 &&
+                                      `(fifo contents0 q0) x0))))
+                              (@PTree.Leaf global_spec))) (@None global_spec)
+                        (@PTree.Leaf global_spec)) (@None global_spec)
+                     (@PTree.Node global_spec
+                        (@PTree.Node global_spec (@PTree.Leaf global_spec)
+                           (@Some global_spec
+                              (Global_func
+                                 (WITH _ : unit PRE 
+                                  [(1%positive, tptr tvoid),
+                                  (2%positive, tint)]
+                                  PROP  ()
+                                  LOCAL ()
+                                  SEP 
+                                  (`(memory_block Tsh)
+                                     (`force_int (eval_id 2%positive))
+                                     (eval_id 1%positive)) POST  [tvoid]
+                                  (fun _ : environ =>
+                                   @emp mpred Nveric Sveric))))
+                           (@PTree.Node global_spec (@PTree.Leaf global_spec)
+                              (@Some global_spec
+                                 (Global_func
+                                    (WITH  p0 : val * list val, p1 : val PRE 
+                                     [(_Q, tptr t_struct_fifo)]
+                                     (let (q0, contents0) := p0 in
+                                      PROP  ()
+                                      LOCAL  (`(@eq val q0) (eval_id _Q))
+                                      SEP  (`(fifo (p1 :: contents0) q0)))
+                                     POST  [tptr t_struct_elem]
+                                     (let (q0, contents0) := p0 in
+                                      fun rho : environ =>
+                                      local (`(@eq val p1) retval) rho &&
+                                      `(fifo contents0 q0) rho *
+                                      `link_ retval rho))))
+                              (@PTree.Leaf global_spec)))
+                        (@Some global_spec
+                           (Global_func
+                              (WITH _ : unit PRE  [(1%positive, tdouble)]
+                               (fun _ : environ => !!False) POST  [tdouble]
+                               (fun _ : environ => !!False))))
+                        (@PTree.Node global_spec (@PTree.Leaf global_spec)
+                           (@None global_spec)
+                           (@PTree.Node global_spec (@PTree.Leaf global_spec)
+                              (@Some global_spec
+                                 (Global_func
+                                    (WITH u : unit PRE  []main_pre prog u
+                                     POST  [tint]main_post prog u)))
+                              (@PTree.Leaf global_spec)))))))) in
+      PROP  ()
+      LOCAL  (tc_environ Delta; `(@eq val tl) (eval_id _t);
+      `(typed_false
+          (typeof
+             (Ebinop Oeq (Etempvar _h (tptr t_struct_elem))
+                (Ecast (Econst_int (Int.repr 0) tint) (tptr tvoid)) tint)))
+        (eval_expr
+           (Ebinop Oeq (Etempvar _h (tptr t_struct_elem))
+              (Ecast (Econst_int (Int.repr 0) tint) (tptr tvoid)) tint));
+      `(@eq val hd) (eval_id _h); `(@eq val q) (eval_id _Q);
+      `(@eq val p) (eval_id _p))
+      SEP 
+      (@numbd (LiftEnviron mpred) 0
+         `(@links t_struct_elem _next QS Tsh prefix hd tl);
+      `(@numbd (lift_T (Tarrow val (Tarrow val (LiftEnviron mpred)))) 1
+          (field_mapsto Tsh
+             (Tstruct _struct_elem
+                (Fcons _a tint
+                   (Fcons _b tint
+                      (Fcons _next (Tcomp_ptr _struct_elem noattr) Fnil)))
+                noattr) _next))
+        (eval_lvalue
+           (Ederef (Etempvar _t (tptr t_struct_elem)) t_struct_elem))
+        (`(eval_cast (typeof (Etempvar _p (tptr t_struct_elem)))
+             (tptr t_struct_elem))
+           (eval_expr (Etempvar _p (tptr t_struct_elem))));
+      @numbd (LiftEnviron mpred) 2
+        `(field_mapsto Tsh t_struct_fifo _head q hd);
+      @numbd (LiftEnviron mpred) 3
+        `(field_mapsto Tsh t_struct_fifo _tail q tl);
+      `(@numbd (lift_T (Tarrow val (Tarrow val (LiftEnviron mpred)))) 4
+          (field_mapsto Tsh
+             (Tstruct _struct_elem
+                (Fcons _a tint
+                   (Fcons _b tint
+                      (Fcons _next (Tcomp_ptr _struct_elem noattr) Fnil)))
+                noattr) _next)) (`force_ptr (eval_id _p))
+        `(Vint (Int.repr 0)))
+      |-- `(@numbd (val -> mpred) n0
+              (field_mapsto_ sh
+                 (typeof
+                    (Ederef (Etempvar _Q (tptr t_struct_fifo)) t_struct_fifo))
+                 _tail))
+            (eval_lvalue
+               (Ederef (Etempvar _Q (tptr t_struct_fifo)) t_struct_fifo)) *
+          @TT (LiftEnviron mpred) (@LiftNatDed' mpred Nveric)))
+. Proof. intros Q p' h t; ungather_entail.
+unfold sh,n0; entailer; cancel.
+Qed.
+
+Lemma goal_13 :
+name _Q ->
+name _p ->
+name _h ->
+name _t ->
+forall (q : val) (contents : list val) (p hd tl : val),
+contents <> @nil val ->
+forall prefix : list val,
+contents = prefix ++ tl :: @nil val ->
+let Delta :=
+  @abbreviate tycontext
+    (initialized _t
+       (initialized _h
+          (@PTree.Node (type * bool)
+             (@PTree.Node (type * bool) (@PTree.Leaf (type * bool))
+                (@None (type * bool))
+                (@PTree.Node (type * bool) (@PTree.Leaf (type * bool))
+                   (@None (type * bool))
+                   (@PTree.Node (type * bool)
+                      (@PTree.Node (type * bool) (@PTree.Leaf (type * bool))
+                         (@Some (type * bool) (tptr t_struct_elem, false))
+                         (@PTree.Leaf (type * bool))) (@None (type * bool))
+                      (@PTree.Leaf (type * bool))))) (@None (type * bool))
+             (@PTree.Node (type * bool)
+                (@PTree.Node (type * bool) (@PTree.Leaf (type * bool))
+                   (@None (type * bool))
+                   (@PTree.Node (type * bool)
+                      (@PTree.Node (type * bool) (@PTree.Leaf (type * bool))
+                         (@Some (type * bool) (tptr t_struct_elem, true))
+                         (@PTree.Leaf (type * bool))) (@None (type * bool))
+                      (@PTree.Leaf (type * bool)))) (@None (type * bool))
+                (@PTree.Node (type * bool)
+                   (@PTree.Node (type * bool)
+                      (@PTree.Node (type * bool) (@PTree.Leaf (type * bool))
+                         (@Some (type * bool) (tptr t_struct_fifo, true))
+                         (@PTree.Leaf (type * bool))) (@None (type * bool))
+                      (@PTree.Leaf (type * bool))) (@None (type * bool))
+                   (@PTree.Node (type * bool)
+                      (@PTree.Node (type * bool) (@PTree.Leaf (type * bool))
+                         (@Some (type * bool) (tptr t_struct_elem, false))
+                         (@PTree.Leaf (type * bool))) (@None (type * bool))
+                      (@PTree.Leaf (type * bool))))), PTree.empty type,
+          tvoid,
+          @PTree.Node global_spec
+            (@PTree.Node global_spec
+               (@PTree.Node global_spec
+                  (@PTree.Node global_spec (@PTree.Leaf global_spec)
+                     (@Some global_spec
+                        (Global_func
+                           (WITH _ : unit PRE  [(1%positive, tptr tvoid),
+                            (2%positive, tptr tvoid), (3%positive, tuint),
+                            (4%positive, tuint)](fun _ : environ => !!False)
+                            POST  [tvoid](fun _ : environ => !!False))))
+                     (@PTree.Node global_spec (@PTree.Leaf global_spec)
+                        (@Some global_spec
+                           (Global_func
+                              (WITH  p0 : val * list val, p1 : val PRE 
+                               [(_Q, tptr t_struct_fifo),
+                               (_p, tptr t_struct_elem)]
+                               (let (q0, contents0) := p0 in
+                                PROP  ()
+                                LOCAL  (`(@eq val q0) (eval_id _Q);
+                                `(@eq val p1) (eval_id _p))
+                                SEP  (`(fifo contents0 q0); `(link_ p1)))
+                               POST  [tvoid]
+                               (let (q0, contents0) := p0 in
+                                `(fifo (contents0 ++ p1 :: @nil val) q0)))))
+                        (@PTree.Leaf global_spec))) (@None global_spec)
+                  (@PTree.Node global_spec
+                     (@PTree.Node global_spec (@PTree.Leaf global_spec)
+                        (@Some global_spec
+                           (Global_func
+                              (WITH _ : unit PRE  []
+                               (fun _ : environ => @emp mpred Nveric Sveric)
+                               POST  [tptr t_struct_fifo]
+                               `(fifo (@nil val)) retval)))
+                        (@PTree.Leaf global_spec)) (@None global_spec)
+                     (@PTree.Node global_spec (@PTree.Leaf global_spec)
+                        (@Some global_spec
+                           (Global_func
+                              (WITH  a : int, b : int PRE  [(_a, tint),
+                               (_b, tint)]
+                               PROP  ()
+                               LOCAL  (`(@eq val (Vint a)) (eval_id _a);
+                               `(@eq val (Vint b)) (eval_id _b))  SEP() POST 
+                               [tptr t_struct_elem]`(elemrep (a, b)) retval)))
+                        (@PTree.Leaf global_spec)))) (@None global_spec)
+               (@PTree.Node global_spec
+                  (@PTree.Node global_spec (@PTree.Leaf global_spec)
+                     (@Some global_spec
+                        (Global_func
+                           (WITH n0 : int PRE  [(1%positive, tint)]
+                            PROP  (4 <= Int.signed n0)
+                            LOCAL 
+                            (`(@eq val (Vint n0)) (eval_id 1%positive))
+                            SEP() POST  [tptr tvoid]
+                            `(memory_block Tsh n0) retval)))
+                     (@PTree.Leaf global_spec)) (@None global_spec)
+                  (@PTree.Leaf global_spec))) (@None global_spec)
+            (@PTree.Node global_spec
+               (@PTree.Node global_spec
+                  (@PTree.Node global_spec (@PTree.Leaf global_spec)
+                     (@Some global_spec
+                        (Global_func
+                           (WITH _ : unit PRE  [(1%positive, tptr tschar),
+                            (2%positive, tint)](fun _ : environ => !!False)
+                            POST  [tint](fun _ : environ => !!False))))
+                     (@PTree.Node global_spec (@PTree.Leaf global_spec)
+                        (@Some global_spec
+                           (Global_func
+                              (WITH  q0 : val, contents0 : list val PRE 
+                               [(_Q, tptr t_struct_fifo)]
+                               PROP  ()
+                               LOCAL  (`(@eq val q0) (eval_id _Q))
+                               SEP  (`(fifo contents0 q0)) POST  [tint]
+                               (fun x0 : environ =>
+                                local
+                                  (`(@eq val
+                                       (if @isnil val contents0
+                                        then Vtrue
+                                        else Vfalse)) retval) x0 &&
+                                `(fifo contents0 q0) x0))))
+                        (@PTree.Leaf global_spec))) (@None global_spec)
+                  (@PTree.Leaf global_spec)) (@None global_spec)
+               (@PTree.Node global_spec
+                  (@PTree.Node global_spec (@PTree.Leaf global_spec)
+                     (@Some global_spec
+                        (Global_func
+                           (WITH _ : unit PRE  [(1%positive, tptr tvoid),
+                            (2%positive, tint)]
+                            PROP  ()
+                            LOCAL ()
+                            SEP 
+                            (`(memory_block Tsh)
+                               (`force_int (eval_id 2%positive))
+                               (eval_id 1%positive)) POST  [tvoid]
+                            (fun _ : environ => @emp mpred Nveric Sveric))))
+                     (@PTree.Node global_spec (@PTree.Leaf global_spec)
+                        (@Some global_spec
+                           (Global_func
+                              (WITH  p0 : val * list val, p1 : val PRE 
+                               [(_Q, tptr t_struct_fifo)]
+                               (let (q0, contents0) := p0 in
+                                PROP  ()
+                                LOCAL  (`(@eq val q0) (eval_id _Q))
+                                SEP  (`(fifo (p1 :: contents0) q0))) POST 
+                               [tptr t_struct_elem]
+                               (let (q0, contents0) := p0 in
+                                fun rho : environ =>
+                                local (`(@eq val p1) retval) rho &&
+                                `(fifo contents0 q0) rho * `link_ retval rho))))
+                        (@PTree.Leaf global_spec)))
+                  (@Some global_spec
+                     (Global_func
+                        (WITH _ : unit PRE  [(1%positive, tdouble)]
+                         (fun _ : environ => !!False) POST  [tdouble]
+                         (fun _ : environ => !!False))))
+                  (@PTree.Node global_spec (@PTree.Leaf global_spec)
+                     (@None global_spec)
+                     (@PTree.Node global_spec (@PTree.Leaf global_spec)
+                        (@Some global_spec
+                           (Global_func
+                              (WITH u : unit PRE  []main_pre prog u POST 
+                               [tint]main_post prog u)))
+                        (@PTree.Leaf global_spec)))))))) in
+PROP  ()
+LOCAL  (tc_environ Delta; `(@eq val tl) (eval_id _t);
+`(typed_false
+    (typeof
+       (Ebinop Oeq (Etempvar _h (tptr t_struct_elem))
+          (Ecast (Econst_int (Int.repr 0) tint) (tptr tvoid)) tint)))
+  (eval_expr
+     (Ebinop Oeq (Etempvar _h (tptr t_struct_elem))
+        (Ecast (Econst_int (Int.repr 0) tint) (tptr tvoid)) tint));
+`(@eq val hd) (eval_id _h); `(@eq val q) (eval_id _Q);
+`(@eq val p) (eval_id _p))
+SEP  (`(@links t_struct_elem _next QS Tsh prefix hd tl);
+`(field_mapsto Tsh
+    (Tstruct _struct_elem
+       (Fcons _a tint
+          (Fcons _b tint (Fcons _next (Tcomp_ptr _struct_elem noattr) Fnil)))
+       noattr) _next)
+  (eval_lvalue (Ederef (Etempvar _t (tptr t_struct_elem)) t_struct_elem))
+  (`(eval_cast (typeof (Etempvar _p (tptr t_struct_elem)))
+       (tptr t_struct_elem)) (eval_expr (Etempvar _p (tptr t_struct_elem))));
+`(field_mapsto Tsh t_struct_fifo _head q hd);
+`(field_mapsto Tsh
+    (Tstruct _struct_fifo
+       (Fcons _head
+          (tptr
+             (Tstruct _struct_elem
+                (Fcons _a tint
+                   (Fcons _b tint
+                      (Fcons _next (Tcomp_ptr _struct_elem noattr) Fnil)))
+                noattr))
+          (Fcons _tail
+             (tptr
+                (Tstruct _struct_elem
+                   (Fcons _a tint
+                      (Fcons _b tint
+                         (Fcons _next (Tcomp_ptr _struct_elem noattr) Fnil)))
+                   noattr)) Fnil)) noattr) _tail)
+  (eval_lvalue (Ederef (Etempvar _Q (tptr t_struct_fifo)) t_struct_fifo))
+  (`(eval_cast (typeof (Etempvar _p (tptr t_struct_elem)))
+       (tptr t_struct_elem)) (eval_expr (Etempvar _p (tptr t_struct_elem))));
+`(field_mapsto Tsh
+    (Tstruct _struct_elem
+       (Fcons _a tint
+          (Fcons _b tint (Fcons _next (Tcomp_ptr _struct_elem noattr) Fnil)))
+       noattr) _next) (`force_ptr (eval_id _p)) `(Vint (Int.repr 0)))
+|-- overridePost
+      (PROP  ()  LOCAL ()  SEP  (`(fifo (contents ++ p :: @nil val) q)))
+      (function_body_ret_assert tvoid `(fifo (contents ++ p :: @nil val) q))
+      EK_normal (@None val)
+. Proof. intros Q p' h t; ungather_entail.
+     entailer.
+     unfold fifo.
+     apply exp_right with (h, p').
+     destruct (isnil ((prefix ++ t :: nil) ++ p' :: nil)).
+     destruct prefix; inv e.
+     normalize.
+     apply exp_right with (prefix ++ t :: nil).
+     entailer.
+     remember (link p' nullval) as A. (* prevent it from canceling! *)
+     cancel. subst. 
+     eapply derives_trans; [ | apply links_cons_right ].
+     cancel.
+Qed.
+
+
